insert fsub.v in dsub.v

dev2016/dsub.v
@@ -3,3 +3,2790 @@
  T ::= Top | x.Type | { Type = T } | { Type <: T } | (z: T) -> T^z
  t ::= x | { Type = T } | lambda x:T.t | t t
 *)
+
+(*
+FSub (F<:)
+T ::= Top | X | T -> T | Forall Z <: T. T^Z
+t ::= x | lambda x:T.t | Lambda X<:T.t | t t | t [T]
+*)
+
+Require Export SfLib.
+
+Require Export Arith.EqNat.
+Require Export Arith.Le.
+Require Import Coq.Program.Equality.
+
+(* ### Syntax ### *)
+
+Definition id := nat.
+
+Inductive ty : Type :=
+| TTop : ty
+| TFun : ty -> ty -> ty
+| TAll : ty -> ty -> ty
+| TVarF : id -> ty (* free type variable, in concrete environment *)
+| TVarH : id -> ty (* free type variable, in abstract environment  *)
+| TVarB : id -> ty (* locally-bound type variable *)
+(* For uniformity, we use TMem to mark type variables in the environment. *)
+(* The advantage is that we don't need to represent two kinds of bindings
+   x: T, X <: T
+   in environments, but instead just
+   x: T, X: TMem T
+*)
+| TMem : ty -> ty  (* Z <: T *)
+.
+
+Inductive tm : Type :=
+| tvar : id -> tm
+| tabs : ty -> tm -> tm
+| tapp : tm -> tm -> tm
+| ttabs : ty -> tm -> tm
+| ttapp : tm -> ty -> tm
+.
+
+Inductive vl : Type :=
+(* a closure for a term abstraction *)
+| vabs : list vl (*H*) -> ty -> tm -> vl
+(* a closure for a type abstraction *)
+| vtabs : list vl (*H*) -> ty -> tm -> vl
+(* For uniformity, we represent a type closing over H here as well,
+   because such types can be bound in H during type application.
+   They represent a type variable binding in the runtime environment,
+   corresponding to TMem in the static environment.
+*)
+| vty : list vl (*H*) -> ty -> vl
+.
+
+Definition tenv := list ty. (* Gamma environment: static *)
+Definition venv := list vl. (* H environment: run-time *)
+Definition aenv := list (venv*ty). (* J environment: abstract at run-time *)
+
+(* ### Representation of Bindings ### *)
+
+(* An environment is a list of values, indexed by decrementing ids. *)
+
+Fixpoint indexr {X : Type} (n : id) (l : list X) : option X :=
+  match l with
+    | [] => None
+    | a :: l' =>
+      if (beq_nat n (length l')) then Some a else indexr n l'
+  end.
+
+Inductive closed: nat(*B*) -> nat(*H*) -> nat(*F*) -> ty -> Prop :=
+| cl_top: forall i j k,
+    closed i j k TTop
+| cl_fun: forall i j k T1 T2,
+    closed i j k T1 ->
+    closed i j k T2 ->
+    closed i j k (TFun T1 T2)
+| cl_all: forall i j k T1 T2,
+    closed i j k T1 ->
+    closed (S i) j k T2 ->
+    closed i j k (TAll T1 T2)
+| cl_sel: forall i j k x,
+    k > x ->
+    closed i j k (TVarF x)
+| cl_selh: forall i j k x,
+    j > x ->
+    closed i j k (TVarH x)
+| cl_selb: forall i j k x,
+    i > x ->
+    closed i j k (TVarB x)
+| cl_mem: forall i j k T,
+    closed i j k T ->
+    closed i j k (TMem T)
+.
+
+(* open define a locally-nameless encoding wrt to TVarB type variables. *)
+(* substitute type u for all occurrences of (TVarB k) *)
+Fixpoint open_rec (k: nat) (u: ty) (T: ty) { struct T }: ty :=
+  match T with
+    | TTop        => TTop
+    | TFun T1 T2  => TFun (open_rec k u T1) (open_rec k u T2)
+    | TAll T1 T2  => TAll (open_rec k u T1) (open_rec (S k) u T2)
+    | TVarF x => TVarF x
+    | TVarH i => TVarH i
+    | TVarB i => if beq_nat k i then u else TVarB i
+    | TMem T0  => TMem (open_rec k u T0)
+  end.
+
+Definition open u T := open_rec 0 u T.
+
+(* Locally-nameless encoding with respect to varH variables. *)
+Fixpoint subst (U : ty) (T : ty) {struct T} : ty :=
+  match T with
+    | TTop         => TTop
+    | TFun T1 T2   => TFun (subst U T1) (subst U T2)
+    | TAll T1 T2   => TAll (subst U T1) (subst U T2)
+    | TVarB i      => TVarB i
+    | TVarF i      => TVarF i
+    | TVarH i      => if beq_nat i 0 then U else TVarH (i-1)
+    | TMem T0      => TMem (subst U T0)
+  end.
+
+Fixpoint nosubst (T : ty) {struct T} : Prop :=
+  match T with
+    | TTop         => True
+    | TFun T1 T2   => nosubst T1 /\ nosubst T2
+    | TAll T1 T2   => nosubst T1 /\ nosubst T2
+    | TVarB i      => True
+    | TVarF i      => True
+    | TVarH i      => i <> 0
+    | TMem T0      => nosubst T0
+  end.
+
+(* ### Static Subtyping ### *)
+(*
+The first env is for looking up varF variables.
+The first env matches the concrete runtime environment, and is
+extended during type assignment.
+
+The second env is for looking up varH variables.
+The second env matches the abstract runtime environment, and is
+extended during subtyping.
+*)
+Inductive stp: tenv -> tenv -> ty -> ty -> Prop :=
+| stp_top: forall G1 GH T1,
+    closed 0 (length GH) (length G1) T1 ->
+    stp G1 GH T1 TTop
+| stp_fun: forall G1 GH T1 T2 T3 T4,
+    stp G1 GH T3 T1 ->
+    stp G1 GH T2 T4 ->
+    stp G1 GH (TFun T1 T2) (TFun T3 T4)
+| stp_mem: forall G1 GH T1 T2,
+    stp G1 GH T1 T2 ->
+    stp G1 GH (TMem T1) (TMem T2)
+| stp_sel1: forall G1 GH T T2 x,
+    indexr x G1 = Some (TMem T) ->
+    closed 0 0 (length G1) T ->
+    stp G1 GH T T2 ->
+    stp G1 GH (TVarF x) T2
+| stp_selx: forall G1 GH v x,
+    (* This is a bit looser than just being able to select on TMem vars. *)
+    indexr x G1 = Some v ->
+    stp G1 GH (TVarF x) (TVarF x)
+| stp_sela1: forall G1 GH T T2 x,
+    indexr x GH = Some (TMem T) ->
+    closed 0 x (length G1) T ->
+    stp G1 GH T T2 ->
+    stp G1 GH (TVarH x) T2
+| stp_selax: forall G1 GH v x,
+    (* This is a bit looser than just being able to select on TMem vars. *)
+    indexr x GH = Some v  ->
+    stp G1 GH (TVarH x) (TVarH x)
+| stp_all: forall G1 GH T1 T2 T3 T4 x,
+    stp G1 GH T3 T1 ->
+    x = length GH ->
+    closed 1 (length GH) (length G1) T2 ->
+    closed 1 (length GH) (length G1) T4 ->
+    stp G1 ((TMem T3)::GH) (open (TVarH x) T2) (open (TVarH x) T4) ->
+    stp G1 GH (TAll T1 T2) (TAll T3 T4)
+.
+
+(* ### Type Assignment ### *)
+Inductive has_type : tenv -> tm -> ty -> Prop :=
+| t_var: forall x env T1,
+           indexr x env = Some T1 ->
+           stp env [] T1 T1 ->
+           has_type env (tvar x) T1
+| t_app: forall env f x T1 T2,
+           has_type env f (TFun T1 T2) ->
+           has_type env x T1 ->
+           has_type env (tapp f x) T2
+| t_abs: forall env y T1 T2,
+           has_type (T1::env) y T2 ->
+           stp env [] (TFun T1 T2) (TFun T1 T2) ->
+           has_type env (tabs T1 y) (TFun T1 T2)
+| t_tapp: forall env f T11 T12 T,
+           has_type env f (TAll T11 T12) ->
+           T = open T11 T12 ->
+           has_type env (ttapp f T11) T
+| t_tabs: forall env y T1 T2,
+            has_type ((TMem T1)::env) y (open (TVarF (length env)) T2) ->
+           stp env [] (TAll T1 T2) (TAll T1 T2) ->
+           has_type env (ttabs T1 y) (TAll T1 T2)
+| t_sub: forall env e T1 T2,
+           has_type env e T1 ->
+           stp env [] T1 T2 ->
+           has_type env e T2
+.
+
+(* ### Runtime Subtyping ### *)
+(* H1 T1 <: H2 T2 -| J *)
+Inductive stp2: bool (* whether the last rule may not be transitivity *) ->
+                venv -> ty -> venv -> ty -> aenv  ->
+                nat (* derivation size *) ->
+                Prop :=
+| stp2_top: forall G1 G2 GH T n,
+    closed 0 (length GH) (length G1) T ->
+    stp2 true G1 T G2 TTop GH (S n)
+| stp2_fun: forall G1 G2 T1 T2 T3 T4 GH n1 n2,
+    stp2 false G2 T3 G1 T1 GH n1 ->
+    stp2 false G1 T2 G2 T4 GH n2 ->
+    stp2 true G1 (TFun T1 T2) G2 (TFun T3 T4) GH (S (n1 + n2))
+| stp2_mem: forall G1 G2 T1 T2 GH n1,
+    stp2 false G1 T1 G2 T2 GH n1 ->
+    stp2 true G1 (TMem T1) G2 (TMem T2) GH (S n1)
+
+(* concrete type variables *)
+(* vty already marks binding as type binding, so need for additional TMem marker *)
+| stp2_sel1: forall G1 G2 GX TX x T2 GH n1,
+    indexr x G1 = Some (vty GX TX) ->
+    closed 0 0 (length GX) TX ->
+    stp2 true GX TX G2 T2 GH n1 ->
+    stp2 true G1 (TVarF x) G2 T2 GH (S n1)
+| stp2_sel2: forall G1 G2 GX TX x T1 GH n1,
+    indexr x G2 = Some (vty GX TX) ->
+    closed 0 0 (length GX) TX ->
+    stp2 false G1 T1 GX TX GH n1 ->
+    stp2 true G1 T1 G2 (TVarF x) GH (S n1)
+| stp2_selx: forall G1 G2 v x1 x2 GH n,
+    indexr x1 G1 = Some v ->
+    indexr x2 G2 = Some v ->
+    stp2 true G1 (TVarF x1) G2 (TVarF x2) GH (S n)
+
+(* abstract type variables *)
+(* X<:T, one sided *)
+| stp2_sela1: forall G1 G2 GX TX x T2 GH n1,
+    indexr x GH = Some (GX, TX) ->
+    closed 0 x (length GX) TX ->
+    stp2 false GX TX G2 T2 GH n1 ->
+    stp2 true G1 (TVarH x) G2 T2 GH (S n1)
+| stp2_selax: forall G1 G2 v x GH n,
+    indexr x GH = Some v ->
+    stp2 true G1 (TVarH x) G2 (TVarH x) GH (S n)
+
+| stp2_all: forall G1 G2 T1 T2 T3 T4 x GH n1 n2,
+    stp2 false G2 T3 G1 T1 GH n1 ->
+    x = length GH ->
+    closed 1 (length GH) (length G1) T2 ->
+    closed 1 (length GH) (length G2) T4 ->
+    stp2 false G1 (open (TVarH x) T2) G2 (open (TVarH x) T4) ((G2, T3)::GH) n2 ->
+    stp2 true G1 (TAll T1 T2) G2 (TAll T3 T4) GH (S (n1 + n2))
+
+| stp2_wrapf: forall G1 G2 T1 T2 GH n1,
+    stp2 true G1 T1 G2 T2 GH n1 ->
+    stp2 false G1 T1 G2 T2 GH (S n1)
+
+| stp2_transf: forall G1 G2 G3 T1 T2 T3 GH n1 n2,
+    stp2 true G1 T1 G2 T2 GH n1 ->
+    stp2 false G2 T2 G3 T3 GH n2 ->
+    stp2 false G1 T1 G3 T3 GH (S (n1+n2))
+.
+
+(* consistent environment *)
+Inductive wf_env : venv -> tenv -> Prop :=
+| wfe_nil : wf_env nil nil
+| wfe_cons : forall v t vs ts,
+    val_type (v::vs) v t ->
+    wf_env vs ts ->
+    wf_env (cons v vs) (cons t ts)
+
+(* value type assignment *)
+with val_type : venv -> vl -> ty -> Prop :=
+| v_ty: forall env venv tenv T1 TE,
+    wf_env venv tenv ->
+    (exists n, stp2 true venv (TMem T1) env TE [] n) ->
+    val_type env (vty venv T1) TE
+| v_abs: forall env venv tenv x y T1 T2 TE,
+    wf_env venv tenv ->
+    has_type (T1::tenv) y T2 ->
+    length venv = x ->
+    (exists n, stp2 true venv (TFun T1 T2) env TE [] n) ->
+    val_type env (vabs venv T1 y) TE
+| v_tabs: forall env venv tenv x y T1 T2 TE,
+    wf_env venv tenv ->
+    has_type ((TMem T1)::tenv) y (open (TVarF x) T2) ->
+    length venv = x ->
+    (exists n, stp2 true venv (TAll T1 T2) env TE [] n) ->
+    val_type env (vtabs venv T1 y) TE
+.
+
+Inductive wf_envh : venv -> aenv -> tenv -> Prop :=
+| wfeh_nil : forall vvs, wf_envh vvs nil nil
+| wfeh_cons : forall t vs vvs ts,
+    wf_envh vvs vs ts ->
+    wf_envh vvs (cons (vvs,t) vs) (cons (TMem t) ts)
+.
+
+Inductive valh_type : venv -> aenv -> (venv*ty) -> ty -> Prop :=
+| v_tya: forall aenv venv T1,
+    valh_type venv aenv (venv, T1) (TMem T1)
+.
+
+(* ### Evaluation (Big-Step Semantics) ### *)
+
+(*
+None             means timeout
+Some None        means stuck
+Some (Some v))   means result v
+
+Could use do-notation to clean up syntax.
+*)
+
+Fixpoint teval(n: nat)(env: venv)(t: tm){struct n}: option (option vl) :=
+  match n with
+    | 0 => None
+    | S n =>
+      match t with
+        | tvar x     => Some (indexr x env)
+        | tabs T y => Some (Some (vabs env T y))
+        | ttabs T y  => Some (Some (vtabs env T y))
+        | tapp ef ex   =>
+          match teval n env ex with
+            | None => None
+            | Some None => Some None
+            | Some (Some vx) =>
+              match teval n env ef with
+                | None => None
+                | Some None => Some None
+                | Some (Some (vty _ _)) => Some None
+                | Some (Some (vtabs _ _ _)) => Some None
+                | Some (Some (vabs env2 _ ey)) =>
+                  teval n (vx::env2) ey
+              end
+          end
+        | ttapp ef ex   =>
+          match teval n env ef with
+            | None => None
+            | Some None => Some None
+            | Some (Some (vty _ _)) => Some None
+            | Some (Some (vabs _ _ _)) => Some None
+            | Some (Some (vtabs env2 T ey)) =>
+              teval n ((vty env ex)::env2) ey
+          end
+      end
+  end.
+
+(* automation *)
+Hint Unfold venv.
+Hint Unfold tenv.
+
+Hint Unfold open.
+Hint Unfold indexr.
+Hint Unfold length.
+
+Hint Constructors ty.
+Hint Constructors tm.
+Hint Constructors vl.
+
+Hint Constructors closed.
+Hint Constructors has_type.
+Hint Constructors val_type.
+Hint Constructors wf_env.
+Hint Constructors stp.
+Hint Constructors stp2.
+
+Hint Constructors option.
+Hint Constructors list.
+
+Hint Resolve ex_intro.
+
+(* ############################################################ *)
+(* Examples *)
+(* ############################################################ *)
+
+Ltac crush_has_tp :=
+  try solve [eapply stp_selx; compute; eauto; crush_has_tp];
+  try solve [eapply stp_selax; compute; eauto; crush_has_tp];
+  try solve [eapply cl_selb; compute; eauto; crush_has_tp];
+  try solve [(econstructor; compute; eauto; crush_has_tp)].
+
+Ltac crush2 :=
+  try solve [(eapply stp_selx; compute; eauto; crush2)];
+  try solve [(eapply stp_selax; compute; eauto; crush2)];
+  try solve [(eapply stp_sel1; compute; eauto; crush2)];
+  try solve [(eapply stp_sela1; compute; eauto; crush2)];
+  try solve [(eapply cl_selb; compute; eauto; crush2)];
+  try solve [(econstructor; compute; eauto; crush2)];
+  try solve [(eapply t_sub; eapply t_var; compute; eauto; crush2)].
+
+(* define polymorphic identity function *)
+
+Definition polyId := TAll TTop (TFun (TVarB 0) (TVarB 0)).
+
+Example ex1: has_type [] (ttabs TTop (tabs (TVarF 0) (tvar 1))) polyId.
+Proof.
+  crush_has_tp.
+Qed.
+
+(* instantiate it to TTop *)
+Example ex2: has_type [polyId] (ttapp (tvar 0) TTop) (TFun TTop TTop).
+Proof.
+  crush2.
+Qed.
+
+
+(* ############################################################ *)
+(* Proofs *)
+(* ############################################################ *)
+
+Fixpoint tsize(T: ty) :=
+  match T with
+    | TTop => 1
+    | TFun T1 T2 => S (tsize T1 + tsize T2)
+    | TAll T1 T2 => S (tsize T1 + tsize T2)
+    | TVarF _ => 1
+    | TVarH _ => 1
+    | TVarB _ => 1
+    | TMem T0 => S (tsize T0)
+  end.
+
+Lemma open_preserves_size: forall T x j,
+  tsize T = tsize (open_rec j (TVarH x) T).
+Proof.
+  intros T. induction T; intros; simpl; eauto.
+  - simpl. destruct (beq_nat j i); eauto.
+Qed.
+
+(* ## Extension, Regularity ## *)
+
+Lemma wf_length : forall vs ts,
+                    wf_env vs ts ->
+                    (length vs = length ts).
+Proof.
+  intros. induction H. auto.
+  compute. eauto.
+Qed.
+
+Hint Immediate wf_length.
+
+Lemma wfh_length : forall vvs vs ts,
+                    wf_envh vvs vs ts ->
+                    (length vs = length ts).
+Proof.
+  intros. induction H. auto.
+  compute. eauto.
+Qed.
+
+Hint Immediate wfh_length.
+
+Lemma indexr_max : forall X vs n (T: X),
+                       indexr n vs = Some T ->
+                       n < length vs.
+Proof.
+  intros X vs. induction vs.
+  - Case "nil". intros. inversion H.
+  - Case "cons".
+    intros. inversion H.
+    case_eq (beq_nat n (length vs)); intros E2.
+    + SSCase "hit".
+      eapply beq_nat_true in E2. subst n. compute. eauto.
+    + SSCase "miss".
+      rewrite E2 in H1.
+      assert (n < length vs). eapply IHvs. apply H1.
+      compute. eauto.
+Qed.
+
+Lemma le_xx : forall a b,
+                       a <= b ->
+                       exists E, le_lt_dec a b = left E.
+Proof. intros.
+  case_eq (le_lt_dec a b). intros. eauto.
+  intros. omega.
+Qed.
+Lemma le_yy : forall a b,
+                       a > b ->
+                       exists E, le_lt_dec a b = right E.
+Proof. intros.
+  case_eq (le_lt_dec a b). intros. omega.
+  intros. eauto.
+Qed.
+
+Lemma indexr_extend : forall X vs n x (T: X),
+                       indexr n vs = Some T ->
+                       indexr n (x::vs) = Some T.
+
+Proof.
+  intros.
+  assert (n < length vs). eapply indexr_max. eauto.
+  assert (beq_nat n (length vs) = false) as E. eapply beq_nat_false_iff. omega.
+  unfold indexr. unfold indexr in H. rewrite H. rewrite E. reflexivity.
+Qed.
+
+(* splicing -- for stp_extend. *)
+
+Fixpoint splice n (T : ty) {struct T} : ty :=
+  match T with
+    | TTop         => TTop
+    | TFun T1 T2   => TFun (splice n T1) (splice n T2)
+    | TAll T1 T2   => TAll (splice n T1) (splice n T2)
+    | TVarF i      => TVarF i
+    | TVarB i      => TVarB i
+    | TVarH i      => if le_lt_dec n i then TVarH (i+1) else TVarH i
+    | TMem T0      => TMem (splice n T0)
+  end.
+
+Definition spliceat n (V: (venv*ty)) :=
+  match V with
+    | (G,T) => (G,splice n T)
+  end.
+
+Lemma splice_open_permute: forall {X} (G0:list X) T2 n j,
+(open_rec j (TVarH (n + S (length G0))) (splice (length G0) T2)) =
+(splice (length G0) (open_rec j (TVarH (n + length G0)) T2)).
+Proof.
+  intros X G T. induction T; intros; simpl; eauto;
+  try rewrite IHT1; try rewrite IHT2; try rewrite IHT; eauto.
+
+  case_eq (le_lt_dec (length G) i); intros E LE; simpl; eauto.
+  case_eq (beq_nat j i); intros E; simpl; eauto.
+  case_eq (le_lt_dec (length G) (n + length G)); intros EL LE.
+  assert (n + S (length G) = n + length G + 1). omega.
+  rewrite H. eauto.
+  omega.
+Qed.
+
+Lemma indexr_splice_hi: forall G0 G2 x0 v1 T,
+    indexr x0 (G2 ++ G0) = Some T ->
+    length G0 <= x0 ->
+    indexr (x0 + 1) (map (splice (length G0)) G2 ++ v1 :: G0) = Some (splice (length G0) T).
+Proof.
+  intros G0 G2. induction G2; intros.
+  - eapply indexr_max in H. simpl in H. omega.
+  - simpl in H.
+    case_eq (beq_nat x0 (length (G2 ++ G0))); intros E.
+    + rewrite E in H. inversion H. subst. simpl.
+      rewrite app_length in E.
+      rewrite app_length. rewrite map_length. simpl.
+      assert (beq_nat (x0 + 1) (length G2 + S (length G0)) = true). {
+        eapply beq_nat_true_iff. eapply beq_nat_true_iff in E. omega.
+      }
+      rewrite H1. eauto.
+    + rewrite E in H.  eapply IHG2 in H. eapply indexr_extend. eapply H. eauto.
+Qed.
+
+Lemma indexr_spliceat_hi: forall G0 G2 x0 v1 G T,
+    indexr x0 (G2 ++ G0) = Some (G, T) ->
+    length G0 <= x0 ->
+    indexr (x0 + 1) (map (spliceat (length G0)) G2 ++ v1 :: G0) =
+    Some (G, splice (length G0) T).
+Proof.
+  intros G0 G2. induction G2; intros.
+  - eapply indexr_max in H. simpl in H. omega.
+  - simpl in H. destruct a.
+    case_eq (beq_nat x0 (length (G2 ++ G0))); intros E.
+    + rewrite E in H. inversion H. subst. simpl.
+      rewrite app_length in E.
+      rewrite app_length. rewrite map_length. simpl.
+      assert (beq_nat (x0 + 1) (length G2 + S (length G0)) = true). {
+        eapply beq_nat_true_iff. eapply beq_nat_true_iff in E. omega.
+      }
+      rewrite H1. eauto.
+    + rewrite E in H.  eapply IHG2 in H. eapply indexr_extend. eapply H. eauto.
+Qed.
+
+Lemma plus_lt_contra: forall a b,
+  a + b < b -> False.
+Proof.
+  intros a b H. induction a.
+  - simpl in H. apply lt_irrefl in H. assumption.
+  - simpl in H. apply IHa. omega.
+Qed.
+
+Lemma indexr_splice_lo0: forall {X} G0 G2 x0 (T:X),
+    indexr x0 (G2 ++ G0) = Some T ->
+    x0 < length G0 ->
+    indexr x0 G0 = Some T.
+Proof.
+  intros X G0 G2. induction G2; intros.
+  - simpl in H. apply H.
+  - simpl in H.
+    case_eq (beq_nat x0 (length (G2 ++ G0))); intros E.
+    + eapply beq_nat_true_iff in E. subst.
+      rewrite app_length in H0. apply plus_lt_contra in H0. inversion H0.
+    + rewrite E in H. apply IHG2. apply H. apply H0.
+Qed.
+
+Lemma indexr_extend_mult: forall {X} G0 G2 x0 (T:X),
+    indexr x0 G0 = Some T ->
+    indexr x0 (G2++G0) = Some T.
+Proof.
+  intros X G0 G2. induction G2; intros.
+  - simpl. assumption.
+  - simpl.
+    case_eq (beq_nat x0 (length (G2 ++ G0))); intros E.
+    + eapply beq_nat_true_iff in E.
+      apply indexr_max in H. subst.
+      rewrite app_length in H. apply plus_lt_contra in H. inversion H.
+    + apply IHG2. assumption.
+Qed.
+
+Lemma indexr_splice_lo: forall G0 G2 x0 v1 T f,
+    indexr x0 (G2 ++ G0) = Some T ->
+    x0 < length G0 ->
+    indexr x0 (map (splice f) G2 ++ v1 :: G0) = Some T.
+Proof.
+  intros.
+  assert (indexr x0 G0 = Some T). eapply indexr_splice_lo0; eauto.
+  eapply indexr_extend_mult. eapply indexr_extend. eauto.
+Qed.
+
+Lemma indexr_spliceat_lo: forall G0 G2 x0 v1 G T f,
+    indexr x0 (G2 ++ G0) = Some (G, T) ->
+    x0 < length G0 ->
+    indexr x0 (map (spliceat f) G2 ++ v1 :: G0) = Some (G, T).
+Proof.
+  intros.
+  assert (indexr x0 G0 = Some (G, T)). eapply indexr_splice_lo0; eauto.
+  eapply indexr_extend_mult. eapply indexr_extend. eauto.
+Qed.
+
+Lemma closed_splice: forall i j k T n,
+  closed i j k T ->
+  closed i (S j) k (splice n T).
+Proof.
+  intros. induction H; simpl; eauto.
+  case_eq (le_lt_dec n x); intros E LE.
+  apply cl_selh. omega.
+  apply cl_selh. omega.
+Qed.
+
+Lemma map_splice_length_inc: forall G0 G2 v1,
+   (length (map (splice (length G0)) G2 ++ v1 :: G0)) = (S (length (G2 ++ G0))).
+Proof.
+  intros. rewrite app_length. rewrite map_length. induction G2.
+  - simpl. reflexivity.
+  - simpl. eauto.
+Qed.
+
+Lemma map_spliceat_length_inc: forall G0 G2 v1,
+   (length (map (spliceat (length G0)) G2 ++ v1 :: G0)) = (S (length (G2 ++ G0))).
+Proof.
+  intros. rewrite app_length. rewrite map_length. induction G2.
+  - simpl. reflexivity.
+  - simpl. eauto.
+Qed.
+
+Lemma closed_inc_mult: forall i j k T,
+  closed i j k T ->
+  forall i' j' k',
+  i' >= i -> j' >= j -> k' >= k ->
+  closed i' j' k' T.
+Proof.
+  intros i j k T H. induction H; intros; eauto; try solve [constructor; omega].
+  - apply cl_all. apply IHclosed1; omega. apply IHclosed2; omega.
+Qed.
+
+Lemma closed_inc: forall i j k T,
+  closed i j k T ->
+  closed i (S j) k T.
+Proof.
+  intros. apply (closed_inc_mult i j k T H i (S j) k); omega.
+Qed.
+
+Lemma closed_splice_idem: forall i j k T n,
+                            closed i j k T ->
+                            n >= j ->
+                            splice n T = T.
+Proof.
+  intros. induction H; eauto.
+  - (* TFun *) simpl.
+    rewrite IHclosed1. rewrite IHclosed2.
+    reflexivity.
+    assumption. assumption.
+  - (* TAll *) simpl.
+    rewrite IHclosed1. rewrite IHclosed2.
+    reflexivity.
+    assumption. assumption.
+  - (* TVarH *) simpl.
+    case_eq (le_lt_dec n x); intros E LE. omega. reflexivity.
+  - (* TMem *) simpl.
+    rewrite IHclosed.
+    reflexivity. assumption.
+Qed.
+
+Ltac ev := repeat match goal with
+                    | H: exists _, _ |- _ => destruct H
+                    | H: _ /\  _ |- _ => destruct H
+           end.
+
+Lemma stp_closed : forall G GH T1 T2,
+                     stp G GH T1 T2 ->
+                     closed 0 (length GH) (length G) T1 /\ closed 0 (length GH) (length G) T2.
+Proof.
+  intros. induction H;
+    try solve [repeat ev; split; eauto using indexr_max].
+Qed.
+
+Lemma stp_closed2 : forall G1 GH T1 T2,
+                       stp G1 GH T1 T2 ->
+                       closed 0 (length GH) (length G1) T2.
+Proof.
+  intros. apply (proj2 (stp_closed G1 GH T1 T2 H)).
+Qed.
+
+Lemma stp_closed1 : forall G1 GH T1 T2,
+                       stp G1 GH T1 T2 ->
+                       closed 0 (length GH) (length G1) T1.
+Proof.
+  intros. apply (proj1 (stp_closed G1 GH T1 T2 H)).
+Qed.
+
+Lemma stp2_closed: forall G1 G2 T1 T2 GH m n,
+                     stp2 m G1 T1 G2 T2 GH n ->
+                     closed 0 (length GH) (length G1) T1 /\ closed 0 (length GH) (length G2) T2.
+  intros. induction H;
+    try solve [repeat ev; split; eauto using indexr_max].
+Qed.
+
+Lemma stp2_closed2 : forall G1 G2 T1 T2 GH m n,
+                       stp2 m G1 T1 G2 T2 GH n ->
+                       closed 0 (length GH) (length G2) T2.
+Proof.
+  intros. apply (proj2 (stp2_closed G1 G2 T1 T2 GH m n H)).
+Qed.
+
+Lemma stp2_closed1 : forall G1 G2 T1 T2 GH m n,
+                       stp2 m G1 T1 G2 T2 GH n ->
+                       closed 0 (length GH) (length G1) T1.
+Proof.
+  intros. apply (proj1 (stp2_closed G1 G2 T1 T2 GH m n H)).
+Qed.
+
+Lemma closed_upgrade: forall i j k i' T,
+ closed i j k T ->
+ i' >= i ->
+ closed i' j k T.
+Proof.
+ intros. apply (closed_inc_mult i j k T H i' j k); omega.
+Qed.
+
+Lemma closed_upgrade_free: forall i j k j' T,
+ closed i j k T ->
+ j' >= j ->
+ closed i j' k T.
+Proof.
+ intros. apply (closed_inc_mult i j k T H i j' k); omega.
+Qed.
+
+Lemma closed_upgrade_freef: forall i j k k' T,
+ closed i j k T ->
+ k' >= k ->
+ closed i j k' T.
+Proof.
+ intros. apply (closed_inc_mult i j k T H i j k'); omega.
+Qed.
+
+Lemma closed_open: forall i j k TX T, closed (i+1) j k T -> closed i j k TX ->
+  closed i j k (open_rec i TX T).
+Proof.
+  intros. generalize dependent i.
+  induction T; intros; inversion H;
+  try econstructor;
+  try eapply IHT1; eauto; try eapply IHT2; eauto; try eapply IHT; eauto.
+  eapply closed_upgrade. eauto. eauto.
+  - Case "TVarB". simpl.
+    case_eq (beq_nat i0 i); intros E. eauto.
+    econstructor. eapply beq_nat_false_iff in E. omega.
+Qed.
+
+Lemma indexr_has: forall X (G: list X) x,
+  length G > x ->
+  exists v, indexr x G = Some v.
+Proof.
+  intros. remember (length G) as n.
+  generalize dependent x.
+  generalize dependent G.
+  induction n; intros; try omega.
+  destruct G; simpl.
+  - simpl in Heqn. inversion Heqn.
+  - simpl in Heqn. inversion Heqn. subst.
+    case_eq (beq_nat x (length G)); intros E.
+    + eexists. reflexivity.
+    + apply beq_nat_false in E. apply IHn; eauto.
+      omega.
+Qed.
+
+Lemma stp_refl_aux: forall n T G GH,
+  closed 0 (length GH) (length G) T ->
+  tsize T < n ->
+  stp G GH T T.
+Proof.
+  intros n. induction n; intros; try omega.
+  inversion H; subst; eauto;
+  try solve [omega];
+  try solve [simpl in H0; constructor; apply IHn; eauto; try omega];
+  try solve [apply indexr_has in H1; destruct H1; eauto].
+  - simpl in H0.
+    eapply stp_all.
+    eapply IHn; eauto; try omega.
+    reflexivity.
+    assumption.
+    assumption.
+    apply IHn; eauto.
+    simpl. apply closed_open; auto using closed_inc.
+    unfold open. rewrite <- open_preserves_size. omega.
+Qed.
+
+Lemma stp_refl: forall T G GH,
+  closed 0 (length GH) (length G) T ->
+  stp G GH T T.
+Proof.
+  intros. apply stp_refl_aux with (n:=S (tsize T)); eauto.
+Qed.
+
+Definition stpd2 m G1 T1 G2 T2 GH := exists n, stp2 m G1 T1 G2 T2 GH n.
+
+Ltac ep := match goal with
+             | [ |- stp2 ?M ?G1 ?T1 ?G2 ?T2 ?GH ?N ] =>
+               assert (exists (n:nat), stp2 M G1 T1 G2 T2 GH n) as EEX
+           end.
+
+Ltac eu := match goal with
+             | H: stpd2 _ _ _ _ _ _ |- _ =>
+               destruct H as [? H]
+           end.
+
+Hint Unfold stpd2.
+
+Lemma stp2_refl_aux: forall n T G GH,
+  closed 0 (length GH) (length G) T ->
+  tsize T < n ->
+  stpd2 true G T G T GH.
+Proof.
+  intros n. induction n; intros; try omega.
+  inversion H; subst; eauto; try omega; try simpl in H0.
+  - destruct (IHn T1 G GH) as [n1 IH1]; eauto; try omega.
+    destruct (IHn T2 G GH) as [n2 IH2]; eauto; try omega.
+    eexists; constructor; try constructor; eauto.
+  - destruct (IHn T1 G GH) as [n1 IH1]; eauto; try omega.
+    destruct (IHn (open (TVarH (length GH)) T2) G ((G,T1)::GH)); eauto; try omega.
+    simpl. apply closed_open; auto using closed_inc.
+    unfold open. rewrite <- open_preserves_size. omega.
+    eexists; econstructor; try constructor; eauto.
+  - eapply indexr_has in H1. destruct H1 as [v HI].
+    eexists; eapply stp2_selx; eauto.
+  - eapply indexr_has in H1. destruct H1 as [v HI].
+    eexists; eapply stp2_selax; eauto.
+  - destruct (IHn T0 G GH) as [n0 IH0]; eauto; try omega.
+Grab Existential Variables. apply 0. apply 0. apply 0.
+Qed.
+
+Lemma stp2_refl: forall T G GH,
+  closed 0 (length GH) (length G) T ->
+  stpd2 true G T G T GH.
+Proof.
+  intros. apply stp2_refl_aux with (n:=S (tsize T)); eauto.
+Qed.
+
+Lemma stp_splice : forall GX G0 G1 T1 T2 v1,
+   stp GX (G1++G0) T1 T2 ->
+   stp GX ((map (splice (length G0)) G1) ++ v1::G0)
+       (splice (length G0) T1) (splice (length G0) T2).
+Proof.
+  intros GX G0 G1 T1 T2 v1 H. remember (G1++G0) as G.
+  revert G0 G1 HeqG.
+  induction H; intros; subst GH; simpl; eauto.
+  - Case "top".
+    eapply stp_top.
+    rewrite map_splice_length_inc.
+    apply closed_splice.
+    assumption.
+  - Case "sel1".
+    eapply stp_sel1. apply H. assumption.
+    assert (splice (length G0) T=T) as A. {
+      eapply closed_splice_idem. eassumption. omega.
+    }
+    rewrite <- A. apply IHstp. reflexivity.
+  - Case "sela1".
+    case_eq (le_lt_dec (length G0) x); intros E LE.
+    + apply stp_sela1 with (T:=(splice (length G0) T)).
+      assert (TMem (splice (length G0) T)=(splice (length G0) (TMem T))) as B by auto.
+      rewrite B. apply indexr_splice_hi. eauto. eauto.
+      eapply closed_splice in H0. assert (S x = x +1) as A by omega.
+      rewrite <- A. eapply H0.
+      eapply IHstp. eauto.
+    + eapply stp_sela1. eapply indexr_splice_lo. eauto. eauto. eauto. eauto.
+      assert (splice (length G0) T=T) as A. {
+        eapply closed_splice_idem. eassumption. omega.
+      }
+      rewrite <- A. eapply IHstp. eauto.
+  - Case "selax".
+    case_eq (le_lt_dec (length G0) x); intros E LE.
+    + eapply stp_selax.
+      eapply indexr_splice_hi. eassumption. assumption.
+    + eapply stp_selax. eapply indexr_splice_lo. eauto. eauto.
+  - Case "all".
+    eapply stp_all.
+    eapply IHstp1. eauto. eauto. eauto.
+
+    simpl. rewrite map_splice_length_inc. apply closed_splice. assumption.
+
+    simpl. rewrite map_splice_length_inc. apply closed_splice. assumption.
+
+    specialize IHstp2 with (G3:=G0) (G4:=(TMem T3) :: G2).
+    simpl in IHstp2. rewrite app_length. rewrite map_length. simpl.
+    repeat rewrite splice_open_permute with (j:=0). subst x.
+    rewrite app_length in IHstp2. simpl in IHstp2.
+    eapply IHstp2. eauto.
+Qed.
+
+Lemma stp2_splice : forall G1 T1 G2 T2 GH1 GH0 v1 m n,
+   stp2 m G1 T1 G2 T2 (GH1++GH0) n ->
+   stp2 m G1 (splice (length GH0) T1) G2 (splice (length GH0) T2)
+        ((map (spliceat (length GH0)) GH1) ++ v1::GH0) n.
+Proof.
+  intros G1 T1 G2 T2 GH1 GH0 v1 m n H. remember (GH1++GH0) as GH.
+  revert GH0 GH1 HeqGH.
+  induction H; intros; subst GH; simpl; eauto.
+  - Case "top".
+    eapply stp2_top.
+    rewrite map_spliceat_length_inc.
+    apply closed_splice.
+    assumption.
+  - Case "sel1".
+    eapply stp2_sel1. apply H. assumption.
+    assert (splice (length GH0) TX=TX) as A. {
+      eapply closed_splice_idem. eassumption. omega.
+    }
+    rewrite <- A. apply IHstp2.
+    reflexivity.
+  - Case "sel2".
+    eapply stp2_sel2. apply H. assumption.
+    assert (splice (length GH0) TX=TX) as A. {
+      eapply closed_splice_idem. eassumption. omega.
+    }
+    rewrite <- A. apply IHstp2.
+    reflexivity.
+  - Case "sela1".
+    case_eq (le_lt_dec (length GH0) x); intros E LE.
+    + eapply stp2_sela1. eapply indexr_spliceat_hi. apply H. eauto.
+      eapply closed_splice in H0. assert (S x = x +1) by omega. rewrite <- H2.
+      eapply H0.
+      eapply IHstp2. eauto.
+    + eapply stp2_sela1. eapply indexr_spliceat_lo. apply H. eauto. eauto.
+      assert (splice (length GH0) TX=TX) as A. {
+        eapply closed_splice_idem. eassumption. omega.
+      }
+      rewrite <- A. eapply IHstp2. eauto.
+  - Case "selax".
+    case_eq (le_lt_dec (length GH0) x); intros E LE.
+    + destruct v. eapply stp2_selax.
+      eapply indexr_spliceat_hi. apply H. eauto.
+    + destruct v. eapply stp2_selax.
+      eapply indexr_spliceat_lo. apply H. eauto.
+  - Case "all".
+    apply stp2_all with (x:= length GH1 + S (length GH0)).
+    eapply IHstp2_1. reflexivity.
+
+    simpl. rewrite map_spliceat_length_inc. rewrite app_length. omega.
+    simpl. rewrite map_spliceat_length_inc. apply closed_splice. assumption.
+    simpl. rewrite map_spliceat_length_inc. apply closed_splice. assumption.
+
+    subst x.
+    specialize IHstp2_2 with (GH2:=GH0) (GH3:=(G2, T3) :: GH1).
+    simpl in IHstp2_2.
+    repeat rewrite splice_open_permute with (j:=0).
+    rewrite app_length in IHstp2_2.
+    eapply IHstp2_2. reflexivity.
+Qed.
+
+Lemma stp_extend : forall G1 GH T1 T2 v1,
+                       stp G1 GH T1 T2 ->
+                       stp G1 (v1::GH) T1 T2.
+Proof.
+  intros. induction H; eauto using indexr_extend, closed_inc.
+  assert (splice (length GH) T2 = T2) as A2. {
+    eapply closed_splice_idem. apply H1. omega.
+  }
+  assert (splice (length GH) T4 = T4) as A4. {
+    eapply closed_splice_idem. apply H2. omega.
+  }
+  assert (TVarH (S (length GH)) = splice (length GH) (TVarH (length GH))) as AH. {
+    simpl. case_eq (le_lt_dec (length GH) (length GH)); intros E LE.
+    simpl. rewrite NPeano.Nat.add_1_r. reflexivity.
+    clear LE. apply lt_irrefl in E. inversion E.
+  }
+  assert (closed 0 (length GH) (length G1) T3). eapply stp_closed1. eauto.
+  assert (splice (length GH) T3 = T3) as A3. {
+    eapply closed_splice_idem. eauto. omega.
+  }
+  assert (map (splice (length GH)) [TMem T3] ++ v1::GH =
+          ((TMem T3)::v1::GH)) as HGX3. {
+    simpl. rewrite A3. eauto.
+  }
+  apply stp_all with (x:=length (v1 :: GH)).
+  apply IHstp1.
+  reflexivity.
+  apply closed_inc. apply H1.
+  apply closed_inc. apply H2.
+  simpl.
+  rewrite <- A2. rewrite <- A4.
+  unfold open.
+  change (TVarH (S (length GH))) with (TVarH (0 + (S (length GH)))).
+  rewrite -> splice_open_permute. rewrite -> splice_open_permute.
+  rewrite <- HGX3.
+  apply stp_splice.
+  simpl. unfold open in H3. rewrite <- H0. apply H3.
+Qed.
+
+Lemma stp_extend_mult : forall G T1 T2 GH GH2,
+                       stp G GH T1 T2 ->
+                       stp G (GH2++GH) T1 T2.
+Proof.
+  intros. induction GH2.
+  - simpl. assumption.
+  - simpl.
+    apply stp_extend. assumption.
+Qed.
+
+Lemma indexr_at_index: forall {A} x0 GH0 GH1 (v:A),
+  beq_nat x0 (length GH1) = true ->
+  indexr x0 (GH0 ++ v :: GH1) = Some v.
+Proof.
+  intros. apply beq_nat_true in H. subst.
+  induction GH0.
+  - simpl. rewrite <- beq_nat_refl. reflexivity.
+  - simpl.
+    rewrite app_length. simpl. rewrite <- plus_n_Sm. rewrite <- plus_Sn_m.
+    rewrite false_beq_nat. assumption. omega.
+Qed.
+
+Lemma indexr_same: forall {A} x0 (v0:A) GH0 GH1 (v:A) (v':A),
+  beq_nat x0 (length GH1) = false ->
+  indexr x0 (GH0 ++ v :: GH1) = Some v0 ->
+  indexr x0 (GH0 ++ v' :: GH1) = Some v0.
+Proof.
+  intros ? ? ? ? ? ? ? E H.
+  induction GH0.
+  - simpl. rewrite E. simpl in H. rewrite E in H. apply H.
+  - simpl.
+    rewrite app_length. simpl.
+    case_eq (beq_nat x0 (length GH0 + S (length GH1))); intros E'.
+    simpl in H. rewrite app_length in H. simpl in H. rewrite E' in H.
+    rewrite H. reflexivity.
+    simpl in H. rewrite app_length in H. simpl in H. rewrite E' in H.
+    rewrite IHGH0. reflexivity. assumption.
+Qed.
+
+Inductive venv_ext : venv -> venv -> Prop :=
+| venv_ext_refl : forall G, venv_ext G G
+| venv_ext_cons : forall T G1 G2, venv_ext G1 G2 -> venv_ext (T::G1) G2.
+
+Inductive aenv_ext : aenv -> aenv -> Prop :=
+| aenv_ext_nil : aenv_ext nil nil
+| aenv_ext_cons :
+    forall T G' G A A',
+      aenv_ext A' A -> venv_ext G' G ->
+      aenv_ext ((G',T)::A') ((G,T)::A).
+
+Lemma aenv_ext_refl: forall GH, aenv_ext GH GH.
+Proof.
+  intros. induction GH.
+  - apply aenv_ext_nil.
+  - destruct a. apply aenv_ext_cons.
+    assumption.
+    apply venv_ext_refl.
+Qed.
+
+Lemma venv_ext__ge_length:
+  forall G G',
+    venv_ext G' G ->
+    length G' >= length G.
+Proof.
+  intros. induction H; simpl; omega.
+Qed.
+
+Lemma aenv_ext__same_length:
+  forall GH GH',
+    aenv_ext GH' GH ->
+    length GH = length GH'.
+Proof.
+  intros. induction H.
+  - simpl. reflexivity.
+  - simpl. rewrite IHaenv_ext. reflexivity.
+Qed.
+
+Lemma indexr_at_ext :
+  forall GH GH' x T G,
+    aenv_ext GH' GH ->
+    indexr x GH = Some (G, T) ->
+    exists G', indexr x GH' = Some (G', T) /\ venv_ext G' G.
+Proof.
+  intros GH GH' x T G Hext Hindex. induction Hext.
+  - simpl in Hindex. inversion Hindex.
+  - simpl. simpl in Hindex.
+    case_eq (beq_nat x (length A)); intros E.
+    rewrite E in Hindex.  inversion Hindex. subst.
+    rewrite <- (@aenv_ext__same_length A A'). rewrite E.
+    exists G'. split. reflexivity. assumption. assumption.
+    rewrite E in Hindex.
+    rewrite <- (@aenv_ext__same_length A A'). rewrite E.
+    apply IHHext. assumption. assumption.
+Qed.
+
+Lemma indexr_extend_venv : forall G G' x T,
+                       indexr x G = Some T ->
+                       venv_ext G' G ->
+                       indexr x G' = Some T.
+Proof.
+  intros G G' x T H HV.
+  induction HV.
+  - assumption.
+  - apply indexr_extend. apply IHHV. apply H.
+Qed.
+
+Lemma stp2_closure_extend_rec:
+  forall G1 G2 T1 T2 GH m n,
+    stp2 m G1 T1 G2 T2 GH n ->
+    (forall G1' G2' GH',
+       aenv_ext GH' GH ->
+       venv_ext G1' G1 ->
+       venv_ext G2' G2 ->
+       stp2 m G1' T1 G2' T2 GH' n).
+Proof.
+  intros G1 G2 T1 T2 GH m n H.
+  induction H; intros; eauto.
+  - Case "top".
+    eapply stp2_top.
+    eapply closed_inc_mult; try eassumption; try omega.
+    rewrite (@aenv_ext__same_length GH GH'). omega. assumption.
+    apply venv_ext__ge_length. assumption.
+  - Case "sel1".
+    eapply stp2_sel1. eapply indexr_extend_venv. apply H.
+    assumption. assumption.
+    apply IHstp2. assumption. apply venv_ext_refl. assumption.
+  - Case "sel2".
+    eapply stp2_sel2. eapply indexr_extend_venv. apply H.
+    assumption. assumption.
+    apply IHstp2. assumption. assumption. apply venv_ext_refl.
+  - Case "selx".
+    eapply stp2_selx.
+    eapply indexr_extend_venv. apply H. assumption.
+    eapply indexr_extend_venv. apply H0. assumption.
+  - Case "sela1".
+    assert (exists GX', indexr x GH' = Some (GX', TX) /\ venv_ext GX' GX) as A. {
+      apply indexr_at_ext with (GH:=GH); assumption.
+    }
+    inversion A as [GX' [H' HX]].
+    apply stp2_sela1 with (GX:=GX') (TX:=TX).
+    assumption.
+    eapply closed_inc_mult; try eassumption; try omega.
+    apply venv_ext__ge_length. assumption.
+    apply IHstp2; assumption.
+  - Case "selax".
+    destruct v as [GX TX].
+    assert (exists GX', indexr x GH' = Some (GX', TX) /\ venv_ext GX' GX) as A. {
+      apply indexr_at_ext with (GH:=GH); assumption.
+    }
+    inversion A as [GX' [H' HX]].
+    apply stp2_selax with (v:=(GX',TX)).
+    assumption.
+  - Case "all".
+    eapply stp2_all with (x:=length GH').
+    apply IHstp2_1; assumption.
+    reflexivity.
+    eapply closed_inc_mult; try eassumption; try omega.
+    rewrite (@aenv_ext__same_length GH GH'). omega. assumption.
+    apply venv_ext__ge_length. assumption.
+    eapply closed_inc_mult; try eassumption; try omega.
+    rewrite (@aenv_ext__same_length GH GH'). omega. assumption.
+    apply venv_ext__ge_length. assumption.
+    subst.  rewrite <- (@aenv_ext__same_length GH GH').
+    apply IHstp2_2. apply aenv_ext_cons.
+    assumption. assumption. assumption. assumption. assumption.
+  - Case "trans".
+    eapply stp2_transf.
+    eapply IHstp2_1.
+    assumption. assumption. apply venv_ext_refl.
+    eapply IHstp2_2.
+    assumption. apply venv_ext_refl. assumption.
+Qed.
+
+Lemma stp2_closure_extend : forall G1 T1 G2 T2 GH GX T v m n,
+                              stp2 m G1 T1 G2 T2 ((GX,T)::GH) n ->
+                              stp2 m G1 T1 G2 T2 ((v::GX,T)::GH) n.
+Proof.
+  intros. eapply stp2_closure_extend_rec. apply H.
+  apply aenv_ext_cons. apply aenv_ext_refl. apply venv_ext_cons.
+  apply venv_ext_refl. apply venv_ext_refl. apply venv_ext_refl.
+Qed.
+
+Lemma stp2_extend : forall v1 G1 G2 T1 T2 H m n,
+                      stp2 m G1 T1 G2 T2 H n ->
+                       stp2 m (v1::G1) T1 G2 T2 H n /\
+                       stp2 m G1 T1 (v1::G2) T2 H n /\
+                       stp2 m (v1::G1) T1 (v1::G2) T2 H n.
+Proof.
+  intros. induction H0;
+    try solve [split; try split; intros; eauto using indexr_extend];
+    try solve [split; try split; intros; constructor; simpl; eauto using indexr_extend, closed_upgrade_freef];
+    try solve [split; try split; intros;
+               inversion IHstp2_1 as [? [? ?]]; inversion IHstp2_2 as [? [? ?]]; eauto];
+    try solve [split; try split; intros; inversion IHstp2 as [? [? ?]]; eauto];
+    try solve [split; try split; intros; inversion IHstp2 as [? [? ?]]; eauto using indexr_extend];
+    try solve [split; try split; intros;
+               inversion IHstp2_1 as [? [? ?]]; inversion IHstp2_2 as [? [? ?]];
+               eauto; eapply stp2_all; simpl; eauto using stp2_closure_extend, closed_upgrade_freef].
+Qed.
+
+Lemma stp2_extend2 : forall v1 G1 G2 T1 T2 H m n,
+                       stp2 m G1 T1 G2 T2 H n ->
+                       stp2 m G1 T1 (v1::G2) T2 H n.
+Proof.
+  intros. apply (proj2 (stp2_extend v1 G1 G2 T1 T2 H m n H0)).
+Qed.
+
+Lemma stp2_extend1 : forall v1 G1 G2 T1 T2 H m n,
+                       stp2 m G1 T1 G2 T2 H n ->
+                       stp2 m (v1::G1) T1 G2 T2 H n.
+Proof.
+  intros. apply (proj1 (stp2_extend v1 G1 G2 T1 T2 H m n H0)).
+Qed.
+
+Lemma stp2_extendH : forall v1 G1 G2 T1 T2 GH m n,
+                       stp2 m G1 T1 G2 T2 GH n ->
+                       stp2 m G1 T1 G2 T2 (v1::GH) n.
+Proof.
+  intros.
+  induction H;
+    try solve [try constructor; simpl; eauto using indexr_extend, closed_upgrade_free];
+    try solve [eapply stp2_transf; simpl; eauto].
+  assert (splice (length GH) T2 = T2) as A2. {
+    eapply closed_splice_idem. apply H1. omega.
+  }
+  assert (splice (length GH) T4 = T4) as A4. {
+    eapply closed_splice_idem. apply H2. omega.
+  }
+  assert (TVarH (S (length GH)) = splice (length GH) (TVarH (length GH))) as AH. {
+    simpl. case_eq (le_lt_dec (length GH) (length GH)); intros E LE.
+    simpl. rewrite NPeano.Nat.add_1_r. reflexivity.
+    clear LE. apply lt_irrefl in E. inversion E.
+  }
+  assert (closed 0 (length GH) (length G2) T3). eapply stp2_closed1. eauto.
+  assert (splice (length GH) T3 = T3) as A3. {
+    eapply closed_splice_idem. eauto. omega.
+  }
+  assert (map (spliceat (length GH)) [(G2, T3)] ++ v1::GH =
+          ((G2, T3)::v1::GH)) as HGX3. {
+    simpl. rewrite A3. eauto.
+  }
+  eapply stp2_all.
+  apply IHstp2_1.
+  reflexivity.
+  apply closed_inc. apply H1.
+  apply closed_inc. apply H2.
+  simpl.
+  rewrite <- A2. rewrite <- A4.
+  unfold open.
+  change (TVarH (S (length GH))) with (TVarH (0 + (S (length GH)))).
+  rewrite -> splice_open_permute.
+  rewrite -> splice_open_permute.
+  rewrite <- HGX3.
+  apply stp2_splice.
+  subst x. simpl. unfold open in H3. apply H3.
+Qed.
+
+Lemma stp2_extendH_mult : forall G1 G2 T1 T2 H H2 m n,
+                       stp2 m G1 T1 G2 T2 H n ->
+                       stp2 m G1 T1 G2 T2 (H2++H) n.
+Proof.
+  intros. induction H2.
+  - simpl. assumption.
+  - simpl.
+    apply stp2_extendH. assumption.
+Qed.
+
+Lemma stp2_extendH_mult0 : forall G1 G2 T1 T2 H2 m n,
+                       stp2 m G1 T1 G2 T2 [] n ->
+                       stp2 m G1 T1 G2 T2 H2 n.
+Proof.
+  intros.
+  assert (H2 = H2++[]) as A by apply app_nil_end. rewrite A.
+  apply stp2_extendH_mult. assumption.
+Qed.
+
+Lemma stp2_reg  : forall G1 G2 T1 T2 GH m n,
+                    stp2 m G1 T1 G2 T2 GH n ->
+                    stpd2 true G1 T1 G1 T1 GH /\ stpd2 true G2 T2 G2 T2 GH.
+Proof.
+  intros.
+  apply stp2_closed in H. destruct H as [H1 H2].
+  split; apply stp2_refl; assumption.
+Qed.
+
+Lemma stp2_reg2 : forall G1 G2 T1 T2 GH m n,
+                       stp2 m G1 T1 G2 T2 GH n ->
+                       stpd2 true G2 T2 G2 T2 GH.
+Proof.
+  intros. apply (proj2 (stp2_reg G1 G2 T1 T2 GH m n H)).
+Qed.
+
+Lemma stp2_reg1 : forall G1 G2 T1 T2 GH m n,
+                       stp2 m G1 T1 G2 T2 GH n ->
+                       stpd2 true G1 T1 G1 T1 GH.
+Proof.
+  intros. apply (proj1 (stp2_reg G1 G2 T1 T2 GH m n H)).
+Qed.
+
+Lemma stp_reg  : forall G GH T1 T2,
+                    stp G GH T1 T2 ->
+                    stp G GH T1 T1 /\ stp G GH T2 T2.
+Proof.
+  intros.
+  apply stp_closed in H. destruct H as [H1 H2].
+  split; apply stp_refl; assumption.
+Qed.
+
+Lemma stp_reg2 : forall G GH T1 T2,
+                       stp G GH T1 T2 ->
+                       stp G GH T2 T2.
+Proof.
+  intros. apply (proj2 (stp_reg G GH T1 T2 H)).
+Qed.
+
+Lemma stp_reg1 : forall G GH T1 T2,
+                       stp G GH T1 T2 ->
+                       stp G GH T1 T1.
+Proof.
+  intros. apply (proj1 (stp_reg G GH T1 T2 H)).
+Qed.
+
+Lemma stpd2_extend2 : forall v1 G1 G2 T1 T2 H m,
+                       stpd2 m G1 T1 G2 T2 H ->
+                       stpd2 m G1 T1 (v1::G2) T2 H.
+Proof.
+  intros. destruct H0 as [n Hsub]. eexists n.
+  apply stp2_extend2; eauto.
+Qed.
+
+Lemma stpd2_extend1 : forall v1 G1 G2 T1 T2 H m,
+                       stpd2 m G1 T1 G2 T2 H ->
+                       stpd2 m (v1::G1) T1 G2 T2 H.
+Proof.
+  intros. destruct H0 as [n Hsub]. eexists n.
+  apply stp2_extend1; eauto.
+Qed.
+
+Lemma stpd2_extendH : forall v1 G1 G2 T1 T2 GH m,
+                       stpd2 m G1 T1 G2 T2 GH ->
+                       stpd2 m G1 T1 G2 T2 (v1::GH).
+Proof.
+  intros. destruct H as [n Hsub]. exists n.
+  apply stp2_extendH; eauto.
+Qed.
+
+Lemma stpd2_extendH_mult : forall G1 G2 T1 T2 GH GH2 m,
+                       stpd2 m G1 T1 G2 T2 GH ->
+                       stpd2 m G1 T1 G2 T2 (GH2++GH).
+Proof.
+  intros. destruct H as [n Hsub]. exists n.
+  apply stp2_extendH_mult; eauto.
+Qed.
+
+Lemma stpd2_closed2 : forall G1 G2 T1 T2 GH m,
+                       stpd2 m G1 T1 G2 T2 GH ->
+                       closed 0 (length GH) (length G2) T2.
+Proof.
+  intros. destruct H as [n Hsub].
+  eapply stp2_closed2; eauto.
+Qed.
+
+Lemma stpd2_closed1 : forall G1 G2 T1 T2 GH m,
+                       stpd2 m G1 T1 G2 T2 GH ->
+                       closed 0 (length GH) (length G1) T1.
+Proof.
+  intros. destruct H as [n Hsub].
+  eapply stp2_closed1; eauto.
+Qed.
+
+Lemma valtp_extend : forall vs v v1 T,
+                       val_type vs v T ->
+                       val_type (v1::vs) v T.
+Proof.
+  intros. induction H; eauto; econstructor; eauto; eapply stpd2_extend2; eauto.
+Qed.
+
+Lemma indexr_safe_ex: forall H1 G1 TF i,
+             wf_env H1 G1 ->
+             indexr i G1 = Some TF ->
+             exists v, indexr i H1 = Some v /\ val_type H1 v TF.
+Proof. intros. induction H.
+   - Case "nil". inversion H0.
+   - Case "cons". inversion H0.
+     case_eq (beq_nat i (length ts)); intros E2.
+     * SSCase "hit".
+       rewrite E2 in H3. inversion H3. subst. clear H3.
+       assert (length ts = length vs). symmetry. eapply wf_length. eauto.
+       simpl. rewrite H2 in E2. rewrite E2.
+       eexists. split. eauto. assumption.
+     * SSCase "miss".
+       rewrite E2 in H3.
+       assert (exists v0,
+                 indexr i vs = Some v0 /\ val_type vs v0 TF). eauto.
+       destruct H2. destruct H2.
+       eexists. split. eapply indexr_extend. eauto.
+       eapply valtp_extend. assumption.
+Qed.
+
+Lemma index_safeh_ex: forall H1 H2 G1 GH TF i,
+             wf_env H1 G1 -> wf_envh H1 H2 GH ->
+             indexr i GH = Some TF ->
+             exists v, indexr i H2 = Some v /\ valh_type H1 H2 v TF.
+Proof. intros. induction H0.
+   - Case "nil". inversion H3.
+   - Case "cons". inversion H3.
+     case_eq (beq_nat i (length ts)); intros E2.
+     * SSCase "hit".
+       rewrite E2 in H2. inversion H2. subst. clear H2.
+       assert (length ts = length vs). symmetry. eapply wfh_length. eauto.
+       simpl. rewrite H1 in E2. rewrite E2.
+       eexists. split. eauto. econstructor.
+     * SSCase "miss".
+       rewrite E2 in H2.
+       assert (exists v : venv * ty,
+                 indexr i vs = Some v /\ valh_type vvs vs v TF). eauto.
+       destruct H1. destruct H1.
+       eexists. split. eapply indexr_extend. eauto.
+       inversion H4. subst.
+       eapply v_tya. (* aenv is not constrained -- bit of a cheat?*)
+Qed.
+
+Inductive res_type: venv -> option vl -> ty -> Prop :=
+| not_stuck: forall venv v T,
+      val_type venv v T ->
+      res_type venv (Some v) T.
+
+Hint Constructors res_type.
+Hint Resolve not_stuck.
+
+(* ### Transitivity ### *)
+
+Definition trans_on Q := forall E F S T,
+  stp E F S Q -> stp E F Q T -> stp E F S T.
+
+Hint Unfold trans_on.
+
+Lemma stp_narrow_aux : forall Q E F G P S T,
+  trans_on Q ->
+  stp E (G ++ [(TMem Q)] ++ F) S T ->
+  stp E F P Q ->
+  stp E (G ++ [(TMem P)] ++ F) S T.
+Proof.
+  intros Q E F G P S T TransQ SsubT PsubQ.
+  dependent induction SsubT; intros; eauto.
+  - apply stp_top.
+    rewrite app_length. rewrite app_length. simpl.
+    rewrite app_length in H. rewrite app_length in H. simpl in H.
+    apply H.
+  - case_eq (beq_nat x (length F)); intros E2.
+    + eapply stp_sela1.
+      eapply indexr_at_index. assumption.
+      eapply beq_nat_true in E2. subst.
+      eapply stp_closed1. eassumption.
+      assert (indexr x (G ++ [TMem Q] ++ F) = Some (TMem Q)) as I. {
+        simpl. apply indexr_at_index. assumption.
+      }
+      rewrite I in H. inversion H. subst.
+      apply TransQ.
+      apply stp_extend_mult. apply stp_extend_mult. assumption.
+      eapply IHSsubT. eassumption. eauto. assumption.
+    + eapply stp_sela1.
+      eapply indexr_same. assumption. eassumption. assumption.
+      eapply IHSsubT. eassumption. eauto. assumption.
+  - case_eq (beq_nat x (length F)); intros E2.
+    + eapply stp_selax.
+      eapply indexr_at_index. assumption.
+    + eapply stp_selax.
+      eapply indexr_same. assumption. eassumption.
+  - assert (length (G ++ [TMem P] ++ F) = length (G ++ [TMem Q] ++ F)) as A. {
+      simpl. rewrite app_length. rewrite app_length. simpl.
+      reflexivity.
+    }
+    eapply stp_all; eauto.
+    rewrite A. assumption.
+    rewrite A. assumption.
+    rewrite A.
+    change (TMem T3 :: G ++ [TMem P] ++ F) with ((TMem T3 :: G) ++ [TMem P] ++ F).
+    eapply IHSsubT2; eauto.
+Qed.
+
+Lemma stp_trans_aux: forall n G GH T1 T2 T3,
+  tsize T2 < n ->
+  stp G GH T1 T2 ->
+  stp G GH T2 T3 ->
+  stp G GH T1 T3.
+Proof.
+  intros n G GH T1 T2 T3 A S12 S23.
+  generalize dependent T3.
+  generalize dependent T1.
+  generalize dependent GH. generalize dependent G.
+  generalize dependent T2.
+  induction n; intros T2 LE G GH T1' S12;
+  induction S12; try discriminate; try inversion LE; subst;
+  intros T3' S23;
+  remember S23 as S23'; clear HeqS23'; inversion S23; subst;
+  eauto 4 using stp_closed1, stp_closed2.
+  - (* TFun - TFun *)
+    eapply stp_fun; eauto.
+    apply (IHn T3). omega. assumption. assumption.
+    apply (IHn T4). omega. assumption. assumption.
+  - (* TAll - TAll *)
+    eapply stp_all; eauto.
+    apply (IHn T3). omega. assumption. assumption.
+    apply (IHn (open (TVarH (length GH)) T4)).
+    unfold open. rewrite <- open_preserves_size. omega.
+    change (TMem T6 :: GH) with ([] ++ [(TMem T6)] ++ GH).
+    apply stp_narrow_aux with (Q:=T3).
+    unfold trans_on.
+    intros. apply (IHn T3). omega. assumption. assumption.
+    simpl. assumption. assumption. assumption.
+Qed.
+
+Lemma stp_trans: forall G GH T1 T2 T3,
+  stp G GH T1 T2 ->
+  stp G GH T2 T3 ->
+  stp G GH T1 T3.
+Proof.
+  intros. eapply (stp_trans_aux (S (tsize T2))); eauto.
+Qed.
+
+Lemma stp_narrow: forall Q E F G P S T,
+  stp E (G ++ [(TMem Q)] ++ F) S T ->
+  stp E F P Q ->
+  stp E (G ++ [(TMem P)] ++ F) S T.
+Proof.
+  intros.
+  apply stp_narrow_aux with (Q:=Q); eauto.
+  unfold trans_on. intros. apply stp_trans with (T2:=Q); eauto.
+Qed.
+
+Lemma stpd2_top: forall G1 G2 GH T,
+    closed 0 (length GH) (length G1) T ->
+    stpd2 true G1 T G2 TTop GH.
+Proof. intros. exists (S 0). eauto. Qed.
+Lemma stpd2_fun: forall G1 G2 T1 T2 T3 T4 GH,
+    stpd2 false G2 T3 G1 T1 GH ->
+    stpd2 false G1 T2 G2 T4 GH ->
+    stpd2 true G1 (TFun T1 T2) G2 (TFun T3 T4) GH.
+Proof. intros. repeat eu. eauto. Qed.
+Lemma stpd2_mem: forall G1 G2 T1 T2 GH,
+    stpd2 false G1 T1 G2 T2 GH ->
+    stpd2 true G1 (TMem T1) G2 (TMem T2) GH.
+Proof. intros. repeat eu. eauto. Qed.
+Lemma stpd2_sel1_down: forall G1 G2 GX TX x T2 GH,
+    indexr x G1 = Some (vty GX TX) ->
+    closed 0 0 (length GX) TX ->
+    stpd2 true GX TX G2 T2 GH ->
+    stpd2 true G1 (TVarF x) G2 T2 GH.
+Proof. intros. repeat eu. eauto. Qed.
+Lemma stpd2_sel2: forall G1 G2 GX TX x T1 GH,
+    indexr x G2 = Some (vty GX TX) ->
+    closed 0 0 (length GX) TX ->
+    stpd2 false G1 T1 GX TX GH ->
+    stpd2 true G1 T1 G2 (TVarF x) GH.
+Proof. intros. repeat eu. eauto. Qed.
+Lemma stpd2_selx: forall G1 G2 v x1 x2 GH,
+    indexr x1 G1 = Some v ->
+    indexr x2 G2 = Some v ->
+    stpd2 true G1 (TVarF x1) G2 (TVarF x2) GH.
+Proof. intros. exists (S 0). eauto. Qed.
+Lemma stpd2_sela1: forall G1 G2 GX TX x T2 GH,
+    indexr x GH = Some (GX, TX) ->
+    closed 0 x (length GX) TX ->
+    stpd2 false GX TX G2 T2 GH ->
+    stpd2 true G1 (TVarH x) G2 T2 GH.
+Proof. intros. repeat eu. eauto. Qed.
+Lemma stpd2_selax: forall G1 G2 v x GH,
+    indexr x GH = Some v ->
+    stpd2 true G1 (TVarH x) G2 (TVarH x) GH.
+Proof. intros. exists (S 0). eauto. Qed.
+Lemma stpd2_all: forall G1 G2 T1 T2 T3 T4 x GH,
+    stpd2 false G2 T3 G1 T1 GH ->
+    x = length GH ->
+    closed 1 (length GH) (length G1) T2 ->
+    closed 1 (length GH) (length G2) T4 ->
+    stpd2 false G1 (open (TVarH x) T2) G2 (open (TVarH x) T4) ((G2, T3)::GH) ->
+    stpd2 true G1 (TAll T1 T2) G2 (TAll T3 T4) GH.
+Proof. intros. repeat eu. eauto. Qed.
+Lemma stpd2_wrapf: forall G1 G2 T1 T2 GH,
+    stpd2 true G1 T1 G2 T2 GH ->
+    stpd2 false G1 T1 G2 T2 GH.
+Proof. intros. repeat eu. eauto. Qed.
+Lemma stpd2_transf: forall G1 G2 G3 T1 T2 T3 GH,
+    stpd2 true G1 T1 G2 T2 GH ->
+    stpd2 false G2 T2 G3 T3 GH ->
+    stpd2 false G1 T1 G3 T3 GH.
+Proof. intros. repeat eu. eauto. Qed.
+
+Lemma stpd2_trans_aux: forall n, forall G1 G2 G3 T1 T2 T3 H n1,
+  stp2 false G1 T1 G2 T2 H n1 -> n1 < n ->
+  stpd2 false G2 T2 G3 T3 H ->
+  stpd2 false G1 T1 G3 T3 H.
+Proof.
+  intros n. induction n; intros; try omega; repeat eu; subst; inversion H0.
+  - Case "wrapf". eapply stpd2_transf; eauto.
+  - Case "transf". eapply stpd2_transf. eauto. eapply IHn. eauto. omega. eauto.
+Qed.
+
+Lemma stpd2_trans: forall G1 G2 G3 T1 T2 T3 H,
+  stpd2 false G1 T1 G2 T2 H ->
+  stpd2 false G2 T2 G3 T3 H ->
+  stpd2 false G1 T1 G3 T3 H.
+Proof. intros. repeat eu. eapply stpd2_trans_aux; eauto. Qed.
+
+Lemma stp2_narrow_aux: forall n, forall m G1 T1 G2 T2 GH n0,
+  stp2 m G1 T1 G2 T2 GH n0 ->
+  n0 <= n ->
+  forall GH1 GH0 GH' GX1 TX1 GX2 TX2,
+    GH=GH1++[(GX2,TX2)]++GH0 ->
+    GH'=GH1++[(GX1,TX1)]++GH0 ->
+    stpd2 false GX1 TX1 GX2 TX2 GH0 ->
+    stpd2 m G1 T1 G2 T2 GH'.
+Proof.
+  intros n.
+  induction n.
+  - Case "z". intros. inversion H0. subst. inversion H; eauto.
+  - Case "s n". intros m G1 T1 G2 T2 GH n0 H NE. inversion H; subst;
+    intros GH1 GH0 GH' GX1 TX1 GX2 TX2 EGH EGH' HX; eauto.
+    + SCase "top". eapply stpd2_top.
+      subst. rewrite app_length. simpl. rewrite app_length in H0. simpl in H0. apply H0.
+    + SCase "fun". eapply stpd2_fun.
+      eapply IHn; try eassumption. omega.
+      eapply IHn; try eassumption. omega.
+    + SCase "mem". eapply stpd2_mem.
+      eapply IHn; try eassumption. omega.
+    + SCase "sel1". eapply stpd2_sel1_down; try eassumption.
+      eapply IHn; try eassumption. omega.
+    + SCase "sel2". eapply stpd2_sel2; try eassumption.
+      eapply IHn; try eassumption. omega.
+    + SCase "sela1".
+      unfold id,venv,aenv in *.
+      case_eq (beq_nat x (length GH0)); intros E.
+      * assert (indexr x ([(GX2, TX2)]++GH0) = Some (GX2, TX2)) as A2. {
+          simpl. rewrite E. reflexivity.
+        }
+        assert (indexr x GH = Some (GX2, TX2)) as A2'. {
+          rewrite EGH. eapply indexr_extend_mult. apply A2.
+        }
+        unfold venv in A2'. rewrite A2' in H0. inversion H0. subst.
+        inversion HX as [nx HX'].
+        eapply stpd2_sela1.
+        eapply indexr_extend_mult. simpl. rewrite E. reflexivity.
+        apply beq_nat_true in E. rewrite E. eapply stp2_closed1. eassumption.
+        eapply stpd2_trans.
+        eexists. eapply stp2_extendH_mult. eapply stp2_extendH_mult. eassumption.
+        eapply IHn; try eassumption. omega.
+        reflexivity. reflexivity.
+      * assert (indexr x GH' = Some (GX, TX)) as A. {
+          subst.
+          eapply indexr_same. apply E. eassumption.
+        }
+        eapply stpd2_sela1. eapply A. assumption.
+        eapply IHn; try eassumption. omega.
+    + SCase "selax".
+      unfold id,venv,aenv in *.
+      case_eq (beq_nat x (length GH0)); intros E.
+      * assert (indexr x ([(GX2, TX2)]++GH0) = Some (GX2, TX2)) as A2. {
+          simpl. rewrite E. reflexivity.
+        }
+        assert (indexr x GH = Some (GX2, TX2)) as A2'. {
+          rewrite EGH. eapply indexr_extend_mult. apply A2.
+        }
+        unfold venv in A2'. rewrite A2' in H0. inversion H0. subst.
+        inversion HX as [nx HX'].
+        eapply stpd2_selax.
+        eapply indexr_extend_mult. simpl. unfold id,venv,aenv in *. rewrite E.
+        reflexivity.
+      * assert (indexr x GH' = Some v) as A. {
+          subst.
+          eapply indexr_same. apply E. eassumption.
+        }
+        eapply stpd2_selax. eapply A.
+    + SCase "all".
+      assert (length GH = length GH') as A. {
+        subst. clear.
+        induction GH1.
+        - simpl. reflexivity.
+        - simpl. simpl in IHGH1. rewrite IHGH1. reflexivity.
+      }
+      eapply stpd2_all.
+      eapply IHn; try eassumption. omega.
+      rewrite <- A. reflexivity.
+      rewrite <- A. assumption. rewrite <- A. assumption.
+      subst.
+      eapply IHn with (GH1:=(G2, T4) :: GH1); try eassumption. omega.
+      simpl. reflexivity. simpl. reflexivity.
+    + SCase "wrapf".
+      eapply stpd2_wrapf.
+      eapply IHn; try eassumption. omega.
+    + SCase "transf".
+      eapply stpd2_transf.
+      eapply IHn; try eassumption. omega.
+      eapply IHn; try eassumption. omega.
+Grab Existential Variables. apply 0.
+Qed.
+
+Lemma stpd2_narrow: forall G1 G2 G3 G4 T1 T2 T3 T4 H,
+  stpd2 false G1 T1 G2 T2 H -> (* careful about H! *)
+  stpd2 false G3 T3 G4 T4 ((G2,T2)::H) ->
+  stpd2 false G3 T3 G4 T4 ((G1,T1)::H).
+Proof.
+  intros. inversion H1 as [n H'].
+  eapply (stp2_narrow_aux n) with (GH1:=[]) (GH0:=H). eapply H'. omega.
+  simpl. reflexivity. reflexivity.
+  assumption.
+Qed.
+
+Ltac indexr_contra :=
+  match goal with
+    | H: indexr ?N [] = Some ?V |- _ => simpl in H; inversion H
+  end.
+
+Lemma stpd2_untrans_aux: forall n, forall m G1 G2 G3 T1 T2 T3 GH n1,
+  stp2 m G1 T1 G2 T2 GH n1 -> n1 < n ->
+  stpd2 true G2 T2 G3 T3 GH ->
+  stpd2 true G1 T1 G3 T3 GH.
+Proof.
+  intros n. induction n; intros; try omega. eu.
+  inversion H; subst;
+  try solve [inversion H1; eexists; eauto];
+  try solve [eapply stpd2_sel1_down; eauto; eapply IHn; eauto; try omega];
+  try solve [eapply stpd2_sela1; eauto; eapply stpd2_wrapf; eapply IHn; eauto; try omega];
+  try solve [eapply IHn; [eapply H2 | omega | eauto]]; (* wrapf *)
+  try solve [eapply IHn; [eapply H2 | omega | (eapply IHn; [ eapply H3 | omega | eauto ])]]; (* transf *)
+  inversion H1; subst;
+  try solve [eapply stpd2_top; eauto using stp2_closed1];
+  try solve [eapply stpd2_sel2; eauto];
+  try solve [eapply stpd2_fun; eapply stpd2_trans; eauto];
+  try solve [eapply stpd2_mem; eauto; eapply stpd2_trans; eauto];
+  try solve [eapply stpd2_sela1; eauto; eapply stpd2_wrapf; eapply IHn; eauto; try omega];
+  try solve [indexr_contra].
+  - Case "sel2 - sel1".
+    rewrite H6 in H2. inversion H2. subst.
+    eapply IHn. eapply H4. omega. eauto.
+  - Case "sel2 - selx".
+    rewrite H6 in H2. inversion H2. subst.
+    eapply stpd2_sel2; eauto.
+  - Case "selx - sel1".
+    rewrite H5 in H3. inversion H3. subst.
+    eapply stpd2_sel1_down; eauto.
+  - Case "selx - selx".
+    rewrite H5 in H3. inversion H3. subst.
+    eapply stpd2_selx; eauto.
+  - Case "selax - selax".
+    eapply stpd2_selax; eauto.
+  - Case "all - all".
+    eapply stpd2_all; eauto.
+    eapply stpd2_trans; eauto.
+    eapply stpd2_trans. eapply stpd2_narrow. eexists. eapply H8. eauto. eauto.
+Grab Existential Variables. apply 0.
+Qed.
+
+Lemma stpd2_upgrade_general: forall G1 G2 T1 T2 GH,
+  stpd2 false G1 T1 G2 T2 GH ->
+  stpd2 true G1 T1 G2 T2 GH.
+Proof.
+  intros. destruct H as [n H].
+  eapply stpd2_untrans_aux; eauto using stp2_reg2.
+Qed.
+
+(* We need to fix stpd2_sel1 to weaken the non-trans hypothesis,
+   that allowed the more convenient one-pass pushback proof. *)
+Lemma stpd2_sel1: forall G1 G2 GX TX x T2 GH,
+    indexr x G1 = Some (vty GX TX) ->
+    closed 0 0 (length GX) TX ->
+    stpd2 false GX TX G2 T2 GH ->
+    stpd2 true G1 (TVarF x) G2 T2 GH.
+Proof.
+  intros. eapply stpd2_sel1_down; eauto using stpd2_upgrade_general.
+Qed.
+
+(* Otherwise, we don't generally need to push back transitivity
+   in non-empty abstract contexts. *)
+Lemma stpd2_untrans: forall G1 G2 G3 T1 T2 T3,
+  stpd2 true G1 T1 G2 T2 [] ->
+  stpd2 true G2 T2 G3 T3 [] ->
+  stpd2 true G1 T1 G3 T3 [].
+Proof. intros. repeat eu. eapply stpd2_untrans_aux; eauto. Qed.
+
+Lemma stpd2_upgrade: forall G1 G2 T1 T2,
+  stpd2 false G1 T1 G2 T2 [] ->
+  stpd2 true G1 T1 G2 T2 [].
+Proof.
+  intros. destruct H as [n H].
+  eapply stpd2_untrans_aux; eauto using stp2_reg2.
+Qed.
+
+(* ### Substitution for relating static and dynamic semantics ### *)
+Lemma indexr_hit2 {X}: forall x (B:X) A G,
+  length G = x ->
+  B = A ->
+  indexr x (B::G) = Some A.
+Proof.
+  intros.
+  unfold indexr.
+  assert (beq_nat x (length G) = true). eapply beq_nat_true_iff. eauto.
+  rewrite H1. subst. reflexivity.
+Qed.
+
+Lemma indexr_miss {X}: forall x (B:X) A G,
+  indexr x (B::G) = A ->
+  x <> (length G)  ->
+  indexr x G = A.
+Proof.
+  intros.
+  unfold indexr in H.
+  assert (beq_nat x (length G) = false). eapply beq_nat_false_iff. eauto.
+  rewrite H1 in H. eauto.
+Qed.
+
+Lemma indexr_hit {X}: forall x (B:X) A G,
+  indexr x (B::G) = Some A ->
+  x = length G ->
+  B = A.
+Proof.
+  intros.
+  unfold indexr in H.
+  assert (beq_nat x (length G) = true). eapply beq_nat_true_iff. eauto.
+  rewrite H1 in H. inversion H. eauto.
+Qed.
+
+Lemma indexr_hit0: forall GH (GX0:venv) (TX0:ty),
+      indexr 0 (GH ++ [(GX0, TX0)]) =
+      Some (GX0, TX0).
+Proof.
+  intros GH. induction GH.
+  - intros. simpl. eauto.
+  - intros. simpl. destruct a. simpl. rewrite app_length. simpl.
+    assert (length GH + 1 = S (length GH)). omega. rewrite H.
+    eauto.
+Qed.
+
+Hint Resolve beq_nat_true_iff.
+Hint Resolve beq_nat_false_iff.
+
+Lemma closed_no_open: forall T x i j k,
+  closed i j k T ->
+  T = open_rec i x T.
+Proof.
+  intros. induction H; intros; eauto;
+  try solve [compute; compute in IHclosed; rewrite <-IHclosed; auto];
+  try solve [compute; compute in IHclosed1; compute in IHclosed2;
+             rewrite <-IHclosed1; rewrite <-IHclosed2; auto].
+
+  Case "TVarB".
+    unfold open_rec. assert (i <> x0). omega.
+    apply beq_nat_false_iff in H0.
+    rewrite H0. auto.
+Qed.
+
+Lemma open_subst_commute: forall T2 TX j k x i,
+closed i j k TX ->
+(open_rec i (TVarH x) (subst TX T2)) =
+(subst TX (open_rec i (TVarH (x+1)) T2)).
+Proof.
+  intros T2 TX j k. induction T2; intros; eauto.
+  -  simpl. rewrite IHT2_1. rewrite IHT2_2. eauto. eauto. eauto.
+  -  simpl. rewrite IHT2_1. rewrite IHT2_2. eauto. eapply closed_upgrade. eauto. eauto. eauto.
+  -  simpl. case_eq (beq_nat i 0); intros E. symmetry. eapply closed_no_open. eauto. simpl. eauto.
+  - simpl. case_eq (beq_nat i0 i); intros E. simpl.
+    assert (x+1<>0). omega. eapply beq_nat_false_iff in H0.
+    assert (x=x+1-1). unfold id. omega.
+    rewrite H0. eauto.
+    simpl. eauto.
+  -  simpl. rewrite IHT2. eauto. eauto.
+Qed.
+
+Lemma closed_no_subst: forall T i k TX,
+   closed i 0 k T ->
+   subst TX T = T.
+Proof.
+  intros T. induction T; intros; inversion H; simpl; eauto;
+  try rewrite (IHT i k TX); eauto; try rewrite (IHT2 (S i) k TX); eauto;
+  try rewrite (IHT1 i k TX); eauto.
+
+  eapply closed_upgrade. eauto. eauto.
+
+  subst. omega.
+Qed.
+
+Lemma closed_subst: forall i j k TX T, closed i (j+1) k T -> closed 0 j k TX -> closed i j k (subst TX T).
+Proof.
+  intros. generalize dependent i.
+  induction T; intros; inversion H;
+  try econstructor;
+  try eapply IHT1; eauto; try eapply IHT2; eauto; try eapply IHT; eauto.
+
+  - Case "TVarH". simpl.
+    case_eq (beq_nat i 0); intros E.
+    eapply closed_upgrade. eapply closed_upgrade_free.
+    eauto. omega. eauto. omega.
+    econstructor. assert (i > 0). eapply beq_nat_false_iff in E. omega. omega.
+Qed.
+
+Lemma subst_open_commute_m: forall i j k j' TX T2, closed (i+1) (j+1) k T2 -> closed 0 j' k TX ->
+    subst TX (open_rec i (TVarH (j+1)) T2) = open_rec i (TVarH j) (subst TX T2).
+Proof.
+  intros. generalize dependent i. generalize dependent j.
+  induction T2; intros; inversion H; simpl; eauto;
+          try rewrite IHT2_1; try rewrite IHT2_2; try rewrite IHT2; eauto.
+
+  - Case "TVarH". simpl. case_eq (beq_nat i 0); intros E.
+    eapply closed_no_open. eapply closed_upgrade. eauto. omega.
+    eauto.
+  - Case "TVarB". simpl. case_eq (beq_nat i0 i); intros E.
+    simpl. case_eq (beq_nat (j+1) 0); intros E2.
+    eapply beq_nat_true_iff in E2. omega.
+    assert (j+1-1 = j). omega. eauto.
+    eauto.
+Qed.
+
+Lemma subst_open_commute: forall i j k TX T2, closed (i+1) (j+1) k T2 -> closed 0 0 k TX ->
+    subst TX (open_rec i (TVarH (j+1)) T2) = open_rec i (TVarH j) (subst TX T2).
+Proof.
+  intros. eapply subst_open_commute_m; eauto.
+Qed.
+
+Lemma subst_open_zero: forall i i' k TX T2, closed i' 0 k T2 ->
+    subst TX (open_rec i (TVarH 0) T2) = open_rec i TX T2.
+Proof.
+  intros. generalize dependent i'. generalize dependent i.
+  induction T2; intros; inversion H; simpl; eauto;
+  try rewrite (IHT2_1 _ i');
+  try rewrite (IHT2_2 _ (S i'));
+  try rewrite (IHT2_2 _ (S i'));
+  try rewrite (IHT2 _ i'); eauto.
+  eapply closed_upgrade; eauto.
+  case_eq (beq_nat i 0); intros E. omega. omega.
+  case_eq (beq_nat i0 i); intros E. eauto. eauto.
+Qed.
+
+Lemma Forall2_length: forall A B f (G1:list A) (G2:list B),
+                        Forall2 f G1 G2 -> length G1 = length G2.
+Proof.
+  intros. induction H.
+  eauto.
+  simpl. eauto.
+Qed.
+
+Lemma nosubst_intro: forall i k T, closed i 0 k T -> nosubst T.
+Proof.
+  intros. generalize dependent i.
+  induction T; intros; inversion H; simpl; eauto.
+  omega.
+Qed.
+
+Lemma nosubst_open: forall i TX T2, nosubst TX -> nosubst T2 -> nosubst (open_rec i TX T2).
+Proof.
+  intros. generalize dependent i. induction T2; intros;
+  try inversion H0; simpl; eauto.
+  case_eq (beq_nat i0 i); intros E. eauto. eauto.
+Qed.
+
+Lemma indexr_subst: forall GH0 x TX T,
+   indexr x (GH0 ++ [(TMem TX)]) = Some T ->
+   x = 0 /\ TMem TX = T \/
+   x > 0 /\ indexr (x-1) (map (subst TX) GH0) = Some (subst TX T).
+Proof.
+  intros GH0. induction GH0; intros.
+  - simpl in H. case_eq (beq_nat x 0); intros E.
+    + rewrite E in H. inversion H.
+      left. split. eapply beq_nat_true_iff. eauto. eauto.
+    + rewrite E in H. inversion H.
+  -  unfold id in H. remember ((length (GH0 ++ [(TMem TX)]))) as L.
+     case_eq (beq_nat x L); intros E.
+     + assert (x = L). eapply beq_nat_true_iff. eauto.
+       eapply indexr_hit in H.
+       right. split. rewrite app_length in HeqL. simpl in HeqL. omega.
+       assert ((x - 1) = (length (map (subst TX) GH0))).
+       rewrite map_length. rewrite app_length in HeqL. simpl in HeqL. unfold id. omega.
+       simpl.
+       eapply beq_nat_true_iff in H1. unfold id in H1. unfold id. rewrite H1.
+       subst. eauto. eauto. subst. eauto.
+     + assert (x <> L). eapply beq_nat_false_iff. eauto.
+       eapply indexr_miss in H. eapply IHGH0 in H.
+       inversion H. left. eapply H1.
+       right. inversion H1. split. eauto.
+       simpl.
+       assert ((x - 1) <> (length (map (subst TX) GH0))).
+       rewrite app_length in HeqL. simpl in HeqL. rewrite map_length.
+       unfold not. intros. subst L. unfold id in H0. unfold id in H2.
+       unfold not in H0. eapply H0. unfold id in H4. rewrite <-H4. omega.
+       eapply beq_nat_false_iff in H4. unfold id in H4. unfold id. rewrite H4.
+       eauto. subst. eauto.
+Qed.
+
+
+Lemma stp_substitute: forall T1 T2 GX GH,
+   stp GX GH T1 T2 ->
+   forall GH0 TX,
+     GH = (GH0 ++ [(TMem TX)]) ->
+     closed 0 0 (length GX) TX ->
+     stp GX (map (subst TX) GH0) TX TX ->
+     stp GX (map (subst TX) GH0)
+         (subst TX T1)
+         (subst TX T2).
+Proof.
+  intros T1 T2 GX GH H.
+  induction H.
+  - Case "top".
+    intros. subst. simpl. rewrite app_length in H. simpl in H.
+    apply stp_top. rewrite map_length.
+    apply closed_subst. assumption.
+    eapply closed_upgrade_free. eassumption. omega.
+  - Case "fun". intros. simpl. eapply stp_fun. eauto. eauto.
+  - Case "mem". intros. simpl. eapply stp_mem. eauto.
+  - Case "sel1". intros. simpl. eapply stp_sel1. apply H. assumption.
+    assert (subst TX T = T) as A. {
+      eapply closed_no_subst. eassumption.
+    }
+    rewrite <- A.
+    apply IHstp; eauto.
+  - Case "selx". intros. simpl. eapply stp_selx. apply H.
+  - Case "sela1". intros GH0 TX ? ? ?. simpl.
+    subst GH. specialize (indexr_subst _ x TX (TMem T) H). intros.
+    destruct H2; destruct H2.
+    + inversion H5. subst. simpl.
+      specialize (IHstp GH0 T).
+      assert (subst T T = T). eapply closed_no_subst; eauto.
+      rewrite H2 in IHstp.
+      eapply IHstp. eauto. eauto. eauto.
+    + subst. simpl.
+      assert (beq_nat x 0 = false). eapply beq_nat_false_iff; omega. rewrite H6. simpl.
+      eapply stp_sela1. simpl in H5. eapply H5.
+      eapply closed_subst.
+      assert (x - 1 + 1 = x) as A by omega.  rewrite A. assumption.
+      eapply closed_upgrade_free. eassumption. omega.
+      eauto.
+  - Case "selax". intros GH0 TX ? ? ?. simpl.
+    subst GH. specialize (indexr_subst _ x TX v H). intros.
+    destruct H0; destruct H0.
+    + subst. simpl. eauto.
+    + subst. simpl. assert (beq_nat x 0 = false). eapply beq_nat_false_iff. omega. rewrite H4. eapply stp_selax. eauto.
+  - Case "all".
+    intros GH0 TX ? ? ?.
+    simpl. eapply stp_all.
+    + eapply IHstp1; eauto.
+    + rewrite map_length. eauto.
+    + rewrite map_length. eapply closed_subst. subst GH.
+      rewrite app_length in H1. simpl in H1. eauto.
+      eapply closed_upgrade_free; eauto. omega.
+    + rewrite map_length. eapply closed_subst. subst GH.
+      rewrite app_length in H2. simpl in H2. eauto.
+      eapply closed_upgrade_free; eauto. omega.
+    + specialize IHstp2 with (GH0:=(TMem T3)::GH0) (TX:=TX).
+      subst GH. simpl in IHstp2.
+      unfold open. unfold open in IHstp2.
+      subst x.
+      rewrite open_subst_commute with (j:=0) (k:=(length G1)).
+      rewrite open_subst_commute with (j:=0) (k:=(length G1)).
+      rewrite app_length in IHstp2. simpl in IHstp2.
+      eapply IHstp2; eauto. eapply stp_extend; eauto.
+      eauto. eauto.
+Qed.
+
+(*
+when and how we can replace with multiple environments:
+
+stp2 G1 T1 G2 T2 (GH0 ++ [(vty GX TX)])
+
+1) T1 closed
+
+   stp2 G1 T1 G2' T2' (subst GH0)
+
+2) G1 contains (GX TX) at some index x1
+
+   index x1 G1 = (GX TX)
+   stp2 G (subst (TVarF x1) T1) G2' T2'
+
+3) G1 = GX
+
+   stp2 G1 (subst TX T1) G2' T2'
+
+4) G1 and GX unrelated
+
+   stp2 ((GX,TX) :: G1) (subst (TVarF (length G1)) T1) G2' T2'
+
+*)
+
+(* ---- two-env substitution. first define what 'compatible' types mean. ---- *)
+
+Definition compat (GX:venv) (TX: ty) (G1:venv) (T1:ty) (T1':ty) :=
+  (exists x1, indexr x1 G1 = Some (vty GX TX) /\ T1' = (subst (TVarF x1) T1)) \/
+  (G1 = GX /\ T1' = (subst TX T1)) \/
+  (closed 0 0 (length G1) T1 /\ T1' = T1) \/ (* this one is for convenience: redundant with next *)
+  (nosubst T1 /\ T1' = subst TTop T1).
+
+
+Definition compat2 (GX:venv) (TX: ty) (p1:(venv*ty)) (p2:(venv*ty)) :=
+  match p1, p2 with
+      (G1,T1), (G2,T2) => G1 = G2 /\ compat GX TX G1 T1 T2
+  end.
+
+Lemma closed_compat: forall GX TX GXX TXX TXX' i j,
+  compat GX TX GXX TXX TXX' ->
+  closed 0 j (length GXX) TX ->
+  closed i (j+1) (length GXX) TXX ->
+  closed i j (length GXX) TXX'.
+Proof.
+  intros. inversion H;[|destruct H2;[|destruct H2]].
+  - destruct H2. destruct H2. rewrite H3.
+    eapply closed_subst. eauto.
+    eapply cl_sel. apply indexr_max in H2. omega.
+  - destruct H2. destruct H2. rewrite H3.
+    eapply closed_subst. eauto. eauto.
+  - destruct H2. rewrite H3.
+    eapply closed_upgrade. eapply closed_upgrade_free. eauto. omega. omega.
+  - destruct H2. rewrite H3.
+    eapply closed_subst. eauto. eauto.
+Qed.
+
+Lemma indexr_compat_miss0: forall GH GH' GX TX (GXX:venv) (TXX:ty) n,
+      Forall2 (compat2 GX TX) GH GH' ->
+      indexr (n+1) (GH ++ [(GX, TX)]) = Some (GXX,TXX) ->
+      exists TXX', indexr n GH' = Some (GXX,TXX') /\ compat GX TX GXX TXX TXX'.
+Proof.
+  intros. revert n H0. induction H.
+  - intros. simpl. eauto. simpl in H0. assert (n+1 <> 0). omega.
+    eapply beq_nat_false_iff in H. rewrite H in H0. inversion H0.
+  - intros. simpl. destruct y.
+    case_eq (beq_nat n (length l')); intros E.
+    + simpl in H1. rewrite app_length in H1. simpl in H1.
+      assert (n = length l'). eapply beq_nat_true_iff. eauto.
+      assert (beq_nat (n+1) (length l + 1) = true). eapply beq_nat_true_iff.
+      rewrite (Forall2_length _ _ _ _ _ H0). omega.
+      rewrite H3 in H1. destruct x. inversion H1. subst. simpl in H.
+      destruct H. subst. eexists. eauto.
+    + simpl in H1. destruct x.
+      assert (n <> length l'). eapply beq_nat_false_iff. eauto.
+      assert (beq_nat (n+1) (length l + 1) = false). eapply beq_nat_false_iff.
+      rewrite (Forall2_length _ _ _ _ _ H0). omega.
+      rewrite app_length in H1. simpl in H1.
+      rewrite H3 in H1.
+      eapply IHForall2. eapply H1.
+Qed.
+
+Lemma compat_top: forall GX TX G1 T1',
+  compat GX TX G1 TTop T1' -> closed 0 0 (length GX) TX -> T1' = TTop.
+Proof.
+  intros ? ? ? ? CC CLX. repeat destruct CC as [|CC]; ev; eauto.
+Qed.
+
+Lemma compat_mem: forall GX TX G1 T1 T1',
+    compat GX TX G1 (TMem T1) T1' ->
+    closed 0 0 (length GX) TX ->
+    exists TA, T1' = TMem TA /\
+                  compat GX TX G1 T1 TA.
+Proof.
+  intros ? ? ? ? ? CC CLX. destruct CC.
+
+  simpl in H. destruct H. destruct H. repeat eexists. eauto. unfold compat. eauto.
+
+  simpl in H. destruct H. destruct H. repeat eexists. eauto. unfold compat. eauto.
+
+  simpl in H. destruct H. destruct H. inversion H. repeat eexists. eauto. unfold compat. eauto.
+
+  simpl in H. destruct H. repeat eexists. eauto. unfold compat. eauto.
+Qed.
+
+Lemma compat_fun: forall GX TX G1 T1 T2 T1',
+    compat GX TX G1 (TFun T1 T2) T1' ->
+    closed 0 0 (length GX) TX ->
+    exists TA TB, T1' = TFun TA TB /\
+                  compat GX TX G1 T1 TA /\
+                  compat GX TX G1 T2 TB.
+Proof.
+  intros ? ? ? ? ? ? CC CLX. destruct CC.
+
+  simpl in H. destruct H. destruct H. repeat eexists. eauto.
+  unfold compat. eauto. unfold compat. eauto.
+
+  simpl in H. destruct H. destruct H. repeat eexists. eauto.
+  unfold compat. eauto. unfold compat. eauto.
+
+  simpl in H. destruct H. destruct H. inversion H. repeat eexists. eauto.
+  unfold compat. eauto. unfold compat. eauto.
+
+  simpl in H. destruct H. destruct H. repeat eexists. eauto.
+  unfold compat. eauto. unfold compat. eauto.
+Qed.
+
+Lemma compat_sel: forall GX TX G1 T1' (GXX:venv) (TXX:ty) x,
+    compat GX TX G1 (TVarF x) T1' ->
+    closed 0 0 (length GX) TX ->
+    closed 0 0 (length GXX) TXX ->
+    indexr x G1 = Some (vty GXX TXX) ->
+    exists TXX', T1' = (TVarF x) /\ compat GX TX GXX TXX TXX'
+.
+Proof.
+  intros ? ? ? ? ? ? ? CC CL CL1 IX.
+
+  destruct CC.
+  destruct H. destruct H. simpl in H0. eexists. split. eauto. right. right. left. eauto.
+  destruct H. destruct H. simpl in H0. eexists. split. eauto. right. right. left. eauto.
+  destruct H. destruct H. simpl in H0. eexists. split. eauto. right. right. left. eauto.
+  destruct H. destruct H. simpl in H0. eexists. split. eauto. right. right. left. eauto.
+Qed.
+
+Lemma compat_selh: forall GX TX G1 T1' GH0 GH0' (GXX:venv) (TXX:ty) x,
+    compat GX TX G1 (TVarH x) T1' ->
+    closed 0 0 (length GX) TX ->
+    indexr x (GH0 ++ [(GX, TX)]) = Some (GXX, TXX) ->
+    Forall2 (compat2 GX TX) GH0 GH0' ->
+    (x = 0 /\ GXX = GX /\ TXX = TX) \/
+    exists TXX',
+      x > 0 /\ T1' = TVarH (x-1) /\
+      indexr (x-1) GH0' = Some (GXX, TXX') /\
+      compat GX TX GXX TXX TXX'
+.
+Proof.
+  intros ? ? ? ? ? ? ? ? ? CC CL IX FA.
+
+  case_eq (beq_nat x 0); intros E.
+  - left. assert (x = 0). eapply beq_nat_true_iff. eauto. subst x.
+    rewrite indexr_hit0 in IX. inversion IX. eauto.
+  - right. assert (x <> 0). eapply beq_nat_false_iff. eauto.
+    assert (x > 0). unfold id. unfold id in H. omega.
+    eapply (indexr_compat_miss0) in FA. destruct FA.
+    destruct CC.
+    + simpl in H2. rewrite E in H2.
+      destruct H2. destruct H2. eexists. eauto.
+    + destruct H2. destruct H2. eexists. eauto. simpl in H3. rewrite E in H3.
+      eauto.
+      destruct H2. destruct H2. inversion H2. subst. omega.
+      destruct H2. simpl in H3. rewrite E in H3. eauto.
+    + assert (x-1+1=x). omega. rewrite H1. eauto.
+Qed.
+
+Lemma compat_all: forall GX TX G1 T1 T2 T1' n,
+    compat GX TX G1 (TAll T1 T2) T1' ->
+    closed 0 0 (length GX) TX -> closed 1 (n+1) (length G1) T2 ->
+    exists TA TB, T1' = TAll TA TB /\
+                  closed 1 n (length G1) TB /\
+                  compat GX TX G1 T1 TA /\
+                  compat GX TX G1 (open_rec 0 (TVarH (n+1)) T2) (open_rec 0 (TVarH n) TB).
+Proof.
+  intros ? ? ? ? ? ? ? CC CLX CL2. destruct CC.
+
+  simpl in H. destruct H. destruct H. repeat eexists. eauto. eapply closed_subst. eauto.
+    apply indexr_max in H. apply cl_sel. omega.
+
+  unfold compat. eauto. unfold compat. left. exists x. split; eauto.
+  erewrite subst_open_commute. eauto. eauto. apply indexr_max in H. eauto.
+
+  destruct H. destruct H. simpl in H0. subst G1.
+  repeat eexists. eauto. eapply closed_subst. eauto.
+  eapply closed_upgrade_free. eauto. omega. unfold compat. eauto. unfold compat.
+  right. left. erewrite subst_open_commute. eauto. eauto. eauto.
+
+  destruct H. destruct H. inversion H. repeat eexists. eauto. subst.
+  eapply closed_upgrade_free. eauto. omega. unfold compat. eauto.
+  unfold compat. eauto. right. right.
+
+  right. split. eapply nosubst_open. simpl. omega. eapply nosubst_intro. eauto. symmetry.
+  assert (T2 = subst TTop T2). symmetry. eapply closed_no_subst. eauto.
+  remember (open_rec 0 (TVarH n) T2) as XX. rewrite H8 in HeqXX. subst XX.
+  eapply subst_open_commute. eauto. eauto.
+
+  simpl in H. destruct H. destruct H. repeat eexists. eauto. eapply closed_subst. eauto. eauto.
+  unfold compat. right. right. right. eauto.
+  unfold compat. right. right. right. split. eapply nosubst_open. simpl. omega. eauto.
+  erewrite subst_open_commute. eauto. eauto. eauto.
+Qed.
+
+Lemma compat_closed: forall GX TX G T T' j,
+  compat GX TX G T T' ->
+  closed 0 (j + 1) (length G) T ->
+  closed 0 0 (length GX) TX ->
+  closed 0 j (length G) T'.
+Proof.
+  intros. inversion H;[|destruct H2;[|destruct H2]].
+  - destruct H2 as [x1 [Hindex Heq]]. subst.
+    apply closed_subst. eassumption.
+    apply indexr_max in Hindex. apply cl_sel. omega.
+  - destruct H2. subst.
+    apply closed_subst. eassumption.
+    eapply closed_upgrade_free. eassumption. omega.
+  - destruct H2. subst.
+    eapply closed_upgrade_free. eapply H2. omega.
+  - destruct H2. subst.
+    apply closed_subst. assumption. eauto.
+Qed.
+
+Lemma stp2_substitute_aux: forall n, forall G1 G2 T1 T2 GH m n1,
+   stp2 m G1 T1 G2 T2 GH n1 ->
+   n1 <= n ->
+   forall GH0 GH0' GX TX T1' T2',
+     GH = (GH0 ++ [(GX, TX)]) ->
+     closed 0 0 (length GX) TX ->
+     compat GX TX G1 T1 T1' ->
+     compat GX TX G2 T2 T2' ->
+     Forall2 (compat2 GX TX) GH0 GH0' ->
+     stpd2 false G1 T1' G2 T2' GH0'.
+Proof.
+  intros n. induction n.
+  Case "z". intros. inversion H0. subst. inversion H; eauto.
+  intros G1 G2 T1 T2 GH m n1 H NE.
+  induction H.
+  - Case "top".
+    intros GH0 GH0' GXX TXX T1' T2' ? CX IX1 IX2 FA; eapply stpd2_wrapf.
+    eapply compat_top in IX2.
+    subst. eapply stpd2_top.
+    eapply compat_closed. eassumption.
+    rewrite app_length in H. simpl in H.
+    erewrite <- Forall2_length. eapply H. eassumption.
+    eassumption. assumption.
+
+  - Case "fun".
+    intros GH0 GH0' GXX TXX T1' T2' ? CX IX1 IX2 FA; eapply stpd2_wrapf.
+    eapply compat_fun in IX1. repeat destruct IX1 as [? IX1].
+    eapply compat_fun in IX2. repeat destruct IX2 as [? IX2].
+    subst. eapply stpd2_fun.
+    eapply IHn; eauto; try omega. eapply IHn; eauto; try omega.
+    eauto. eauto.
+
+  - Case "mem".
+    intros GH0 GH0' GXX TXX T1' T2' ? CX IX1 IX2 FA; eapply stpd2_wrapf.
+    eapply compat_mem in IX1. repeat destruct IX1 as [? IX1].
+    eapply compat_mem in IX2. repeat destruct IX2 as [? IX2].
+    subst. eapply stpd2_mem.
+    eapply IHn; eauto; try omega.
+    eauto. eauto.
+
+  - Case "sel1".
+    intros GH0 GH0' GXX TXX T1' T2' ? CX IX1 IX2 FA; eapply stpd2_wrapf.
+
+    assert (length GH = length GH0 + 1). subst GH. eapply app_length.
+    assert (length GH0 = length GH0') as EL. eapply Forall2_length. eauto.
+
+    eapply (compat_sel GXX TXX G1 T1' GX TX) in IX1. repeat destruct IX1 as [? IX1].
+
+    assert (compat GXX TXX GX TX TX) as CPX. right. right. left. eauto.
+
+    subst.
+    eapply stpd2_sel1; eauto.
+    eapply IHn; eauto; try omega.
+    eauto. eauto. eauto.
+
+  - Case "sel2".
+    intros GH0 GH0' GXX TXX T1' T2' ? CX IX1 IX2 FA; eapply stpd2_wrapf.
+
+    assert (length GH = length GH0 + 1). subst GH. eapply app_length.
+    assert (length GH0 = length GH0') as EL. eapply Forall2_length. eauto.
+
+    eapply (compat_sel GXX TXX G2 T2' GX TX) in IX2. repeat destruct IX2 as [? IX2].
+
+    assert (compat GXX TXX GX TX TX) as CPX. right. right. left. eauto.
+
+    subst.
+    eapply stpd2_sel2; eauto.
+    eapply IHn; eauto; try omega.
+    eauto. eauto. eauto.
+
+  - Case "selx".
+    intros GH0 GH0' GXX TXX T1' T2' ? CX IX1 IX2 FA; eapply stpd2_wrapf.
+
+    assert (length GH = length GH0 + 1). subst GH. eapply app_length.
+    assert (length GH0 = length GH0') as EL. eapply Forall2_length. eauto.
+
+    assert (T1' = TVarF x1). {
+      destruct IX1. ev. eauto.
+      destruct H3. ev. auto.
+      destruct H3. ev. eauto.
+      destruct H3. eauto.
+    }
+    assert (T2' = TVarF x2). {
+      destruct IX2. ev. eauto.
+      destruct H4. ev. auto.
+      destruct H4. ev. eauto.
+      destruct H4. ev. eauto.
+    }
+    subst.
+    eapply stpd2_selx. eauto. eauto.
+
+  - Case "sela1".
+    intros GH0 GH0' GXX TXX T1' T2' ? CX IX1 IX2 FA.
+
+    assert (length GH = length GH0 + 1). subst GH. eapply app_length.
+    assert (length GH0 = length GH0') as EL. eapply Forall2_length. eauto.
+
+    assert (compat GXX TXX G1 (TVarH x) T1') as IXX. eauto.
+
+    eapply (compat_selh GXX TXX G1 T1' GH0 GH0' GX TX) in IX1. repeat destruct IX1 as [? IX1].
+
+    destruct IX1.
+    + SCase "x = 0".
+      repeat destruct IXX as [|IXX]; ev.
+      * subst. simpl.
+        eapply stpd2_wrapf. eapply stpd2_sel1. eauto. eauto.
+        eapply IHn; eauto; try omega. right. right. left. auto.
+      * subst. simpl.
+        eapply IHn; eauto; try omega. right. right. left. auto.
+      * subst. inversion H5. subst. omega.
+      * subst. destruct H5. eauto.
+    + SCase "x > 0".
+      ev. subst.
+      eapply stpd2_wrapf. eapply stpd2_sela1. eauto.
+
+      assert (x-1+1=x) as A by omega.
+      remember (x-1) as x1. rewrite <- A in H0.
+      eapply compat_closed. eauto. eauto. eauto.
+      eapply IHn; eauto; try omega.
+    (* remaining obligations *)
+    + eauto. + subst GH. eauto. + eauto.
+
+  - Case "selax".
+    intros GH0 GH0' GXX TXX T1' T2' ? CX IX1 IX2 FA; eapply stpd2_wrapf.
+
+    assert (length GH = length GH0 + 1). subst GH. eapply app_length.
+    assert (length GH0 = length GH0') as EL. eapply Forall2_length. eauto.
+
+    assert (compat GXX TXX G1 (TVarH x) T1') as IXX1. eauto.
+    assert (compat GXX TXX G2 (TVarH x) T2') as IXX2. eauto.
+
+    destruct v as [GX TX].
+    eapply (compat_selh GXX TXX G1 T1' GH0 GH0' GX TX) in IX1. repeat destruct IX1 as [? IX1].
+    eapply (compat_selh GXX TXX G2 T2' GH0 GH0' GX TX) in IX2. repeat destruct IX2 as [? IX2].
+
+    destruct IX1; destruct IX2.
+    + destruct H3. destruct H4. subst. (* x = 0 *)
+
+      inversion IXX1; inversion IXX2.
+
+      destruct H0. destruct H0. subst. simpl.
+      destruct H3. destruct H3. subst. simpl.
+      eapply stpd2_sel1. eauto. eauto.
+      eapply stpd2_wrapf. eapply stpd2_sel2. eauto. eauto.
+      eapply stpd2_wrapf.
+      eapply stp2_refl. eapply closed_upgrade_free. eassumption. omega.
+
+      destruct H0. destruct H0. subst. simpl.
+      destruct H3. destruct H3. subst. simpl.
+      eapply stpd2_sel1. eauto. eauto.
+      eapply stpd2_wrapf.
+      eapply stp2_refl. eapply closed_upgrade_free. eassumption. omega.
+
+      destruct H3. destruct H3. subst. simpl.
+      inversion H3. omega. (* contra *)
+
+      destruct H3. destruct H3. eauto. (* contra *)
+
+      (* --- *)
+
+      destruct H0. destruct H0. subst. simpl.
+      destruct H3. destruct H0. subst. simpl.
+      eapply stpd2_sel2. eauto. eauto.
+      eapply stpd2_wrapf.
+      eapply stp2_refl. eapply closed_upgrade_free. eassumption. omega.
+
+      destruct H0. destruct H0. inversion H0. omega. (* contra *)
+
+      destruct H0. destruct H0. eauto. (* contra *)
+
+      (* --- *)
+
+      destruct H0. destruct H0. subst. simpl.
+      destruct H3. destruct H0. subst. simpl.
+      eapply stp2_refl. eapply closed_upgrade_free. eassumption. omega.
+
+      destruct H0. destruct H0. inversion H0. omega.
+      destruct H0. destruct H0. eauto.
+      destruct H0. destruct H0. inversion H0. omega.
+      destruct H0. destruct H0. eauto.
+
+    + destruct H3. destruct H3. omega.
+    + destruct H2. destruct H3. omega.
+    + destruct H2. destruct H2. destruct H4. destruct H5.
+      destruct H3. destruct H3. destruct H7. destruct H8.
+      subst. eapply stpd2_selax. eauto.
+
+    + eauto.
+    + subst GH. eauto.
+    + eauto.
+    + eauto.
+    + eauto. subst GH. eauto.
+    + eauto.
+
+  - Case "all".
+    intros GH0 GH0' GX TX T1' T2' ? CX IX1 IX2 FA; eapply stpd2_wrapf.
+
+    assert (length GH = length GH0 + 1). subst GH. eapply app_length.
+    assert (length GH0 = length GH0') as EL. eapply Forall2_length. eauto.
+
+    eapply compat_all in IX1. repeat destruct IX1 as [? IX1].
+    eapply compat_all in IX2. repeat destruct IX2 as [? IX2].
+
+    subst.
+
+    eapply stpd2_all.
+    + eapply IHn; eauto; try omega.
+    + eauto.
+    + eauto.
+    + eauto.
+    + subst.
+      eapply IHn. eauto. omega. simpl.
+      change ((G2, T3) :: GH0 ++ [(GX, TX)]) with (((G2, T3) :: GH0) ++ [(GX, TX)]).
+      reflexivity.
+      eauto.
+      rewrite app_length. simpl. rewrite EL. eauto.
+      rewrite app_length. simpl. rewrite EL. eauto.
+      eapply Forall2_cons. simpl. eauto. eauto.
+    + eauto.
+    + eauto. subst GH. rewrite <-EL. eapply closed_upgrade_free. eauto. omega.
+    + eauto.
+    + eauto. subst GH. rewrite <-EL. eapply closed_upgrade_free. eauto. omega.
+  - Case "wrapf".
+    intros. subst. eapply IHn; eauto; try omega.
+  - Case "transf".
+    intros. subst.
+    apply stp2_extend2 with (v1:=(vty GX TX)) in H.
+    apply stp2_extend1 with (v1:=(vty GX TX)) in H0.
+    eapply stpd2_trans.
+
+    eapply IHn; eauto; try omega.
+    unfold compat. simpl. left. exists (length G2).
+    rewrite <- beq_nat_refl. split; eauto.
+
+    eapply IHn; eauto; try omega.
+    unfold compat. simpl. left. exists (length G2).
+    rewrite <- beq_nat_refl. split; eauto.
+Qed.
+
+Lemma stp2_substitute: forall G1 G2 T1 T2 GH m,
+   stpd2 m G1 T1 G2 T2 GH ->
+   forall GH0 GH0' GX TX T1' T2',
+     GH = (GH0 ++ [(GX, TX)]) ->
+     closed 0 0 (length GX) TX ->
+     compat GX TX G1 T1 T1' ->
+     compat GX TX G2 T2 T2' ->
+     Forall2 (compat2 GX TX) GH0 GH0' ->
+     stpd2 false G1 T1' G2 T2' GH0'.
+Proof.
+  intros. repeat eu. eapply stp2_substitute_aux; eauto.
+Qed.
+
+(* ### Relating Static and Dynamic Subtyping ### *)
+Lemma stp_to_stp2: forall G1 GH T1 T2,
+  stp G1 GH T1 T2 ->
+  forall GX GY, wf_env GX G1 -> wf_envh GX GY GH ->
+  stpd2 false GX T1 GX T2 GY.
+Proof.
+  intros G1 G2 T1 T2 ST. induction ST; intros GX GY WX WY; eapply stpd2_wrapf.
+  - Case "top".
+    eapply stpd2_top. erewrite wfh_length; eauto. erewrite wf_length; eauto.
+  - Case "fun". eapply stpd2_fun; eauto.
+  - Case "mem". eapply stpd2_mem; eauto.
+  - Case "sel1".
+    assert (exists v : vl, indexr x GX = Some v /\ val_type GX v (TMem T)) as A.
+    eapply indexr_safe_ex. eauto. eauto.
+    destruct A as [? [? VT]].
+    inversion VT; subst.
+    destruct H3 as [? H3]. inversion H3. subst.
+    eapply stp2_extendH_mult with (H2:=GY) in H7. rewrite app_nil_r in H7.
+    eapply stpd2_sel1; eauto. inversion H2. subst.
+    eapply stp2_closed1 in H3. eauto. inversion H3. subst. simpl in H9. apply H9.
+    eapply stp2_closed1 in H3. eauto. inversion H3. subst. simpl in H13. apply H13.
+    eapply stpd2_trans. eexists. apply H7. eapply IHST; eauto.
+    destruct H5 as [? H5]. inversion H5.
+    destruct H5 as [? H5]. inversion H5.
+  - Case "selx". eauto.
+    assert (exists v0 : vl, indexr x GX = Some v0 /\ val_type GX v0 v) as A.
+    eapply indexr_safe_ex. eauto. eauto. eauto.
+    destruct A as [? [? ?]].
+    eapply stpd2_selx; eauto.
+  - Case "sela1". eauto.
+    assert (exists v, indexr x GY = Some v /\ valh_type GX GY v (TMem T)) as A.
+    eapply index_safeh_ex. eauto. eauto. eauto.
+    destruct A as [? [? VT]]. destruct x0.
+    inversion VT. subst.
+    eapply stpd2_sela1. eauto.
+    erewrite wf_length; eauto.
+    eapply IHST. eauto. eauto.
+  - Case "selax". eauto.
+    assert (exists v0, indexr x GY = Some v0 /\ valh_type GX GY v0 v) as A.
+    eapply index_safeh_ex. eauto. eauto. eauto.
+    destruct A as [? [? VT]]. destruct x0.
+    destruct VT. subst.
+    eapply stpd2_selax. eauto.
+  - Case "all".
+    subst x.
+    assert (length GY = length GH) as A. eapply wfh_length; eauto.
+    assert (length GX = length G1) as B. eapply wf_length; eauto.
+    eapply stpd2_all. eauto. eauto.
+    rewrite A. rewrite B. eauto.
+    rewrite A. rewrite B. eauto.
+    rewrite A.
+    eapply IHST2. eauto. eapply wfeh_cons. eauto.
+Qed.
+
+Lemma valtp_widen: forall vf H1 H2 T1 T2,
+  val_type H1 vf T1 ->
+  stpd2 true H1 T1 H2 T2 [] ->
+  val_type H2 vf T2.
+Proof.
+  intros. inversion H; econstructor; eauto; eapply stpd2_untrans; eauto.
+Qed.
+
+Lemma restp_widen: forall vf H1 H2 T1 T2,
+  res_type H1 vf T1 ->
+  stpd2 true H1 T1 H2 T2 [] ->
+  res_type H2 vf T2.
+Proof.
+  intros. inversion H. eapply not_stuck. eapply valtp_widen; eauto.
+Qed.
+
+
+(* ### Inversion Lemmas ### *)
+
+Lemma invert_abs: forall venv vf T1 T2,
+  val_type venv vf (TFun T1 T2) ->
+  exists env tenv x y T3 T4,
+    vf = (vabs env T3 y) /\
+    length env = x /\
+    wf_env env tenv /\
+    has_type (T3::tenv) y T4 /\
+    stpd2 true venv T1 env T3 [] /\
+    stpd2 true env T4 venv T2 [].
+Proof.
+  intros. inversion H; repeat ev; try solve by inversion.
+  inversion H3. subst.
+  assert (stpd2 false venv0 T1 venv1 T0 []) as E1. eauto.
+  assert (stpd2 false venv1 T3 venv0 T2 []) as E2. eauto.
+  eapply stpd2_upgrade in E1. eapply stpd2_upgrade in E2.
+  repeat eu. repeat eexists; eauto.
+Qed.
+
+Lemma invert_tabs: forall venv vf T1 T2,
+  val_type venv vf (TAll T1 T2) ->
+  exists env tenv x y T3 T4,
+    vf = (vtabs env T3 y) /\
+    length env = x /\
+    wf_env env tenv /\
+    has_type ((TMem T3)::tenv) y (open (TVarF x) T4) /\
+    stpd2 true venv T1 env T3 [] /\
+    stpd2 true ((vty venv T1)::env) (open (TVarF x) T4) venv (open T1 T2) [].
+Proof.
+  intros. inversion H; ev; try solve by inversion. inversion H3. subst.
+  eexists. eexists. eexists. eexists. eexists. eexists.
+  repeat split; eauto; remember (length venv1) as x.
+
+  eapply stpd2_upgrade; eauto.
+  (* inversion of TAll < TAll *)
+  assert (stpd2 true venv0 T1 venv1 T0 []). eapply stpd2_upgrade; eauto.
+  assert (stpd2 false venv1 (open (TVarH 0) T3) venv0 (open (TVarH 0) T2) [(venv0, T1)]). {
+    eauto.
+  }
+
+  (* need reflexivity *)
+  assert (stpd2 true venv0 T1 venv0 T1 []). eapply stp2_reg1. eauto.
+  assert (closed 0 0 (length venv0) T1). eapply stpd2_closed1 in H5. simpl in H5. eauto.
+
+  (* now rename *)
+
+  assert (stpd2 false ((vty venv0 T1) :: venv1) (open_rec 0 (TVarF x) T3) venv0 (open T1 T2) []). {
+    eapply stp2_substitute with (GH0:=nil).
+    eapply stpd2_extend1. eapply H4. simpl. eauto.
+    simpl. eauto.
+    eauto.
+    left. eexists. split. eapply indexr_hit2. eauto. eauto. eauto. unfold open.
+    erewrite (subst_open_zero 0 1). subst x.
+    assert ((length venv1) + 0=length venv1) as R by omega. rewrite R. eauto. eauto.
+    right. left. split. eauto. unfold open. erewrite (subst_open_zero 0 1). eauto. eauto.
+    eauto.
+  }
+
+  (* done *)
+  subst.
+  eapply stpd2_upgrade; eauto.
+Qed.
+
+(* ### Type Safety ### *)
+(* If term type-checks and the term evaluates without timing-out,
+   the result is not stuck, but a value.
+*)
+Theorem full_safety : forall n e tenv venv res T,
+  teval n venv e = Some res -> has_type tenv e T -> wf_env venv tenv ->
+  res_type venv res T.
+
+Proof.
+  intros n. induction n.
+  (* 0 *)   intros. inversion H.
+  (* S n *) intros. destruct e; inversion H.
+
+  - Case "Var".
+    remember (tvar i) as e. induction H0; inversion Heqe; subst.
+    + destruct (indexr_safe_ex venv0 env T1 i) as [v [I V]]; eauto.
+      rewrite I. eapply not_stuck. eapply V.
+
+    + eapply restp_widen. eapply IHhas_type; eauto.
+      eapply stpd2_upgrade. eapply stp_to_stp2; eauto. econstructor.
+
+  - Case "Abs".
+    remember (tabs t e) as xe. induction H0; inversion Heqxe; subst.
+    + eapply not_stuck. eapply v_abs; eauto.
+      eauto. eapply stpd2_upgrade. eapply stp_to_stp2. eauto. eauto. econstructor.
+    + eapply restp_widen. eapply IHhas_type; eauto.
+      eapply stpd2_upgrade. eapply stp_to_stp2; eauto. econstructor.
+
+  - Case "App".
+    remember (tapp e1 e2) as e. induction H0; inversion Heqe; subst.
+    +
+      remember (teval n venv0 e1) as tf.
+      remember (teval n venv0 e2) as tx.
+
+
+      destruct tx as [rx|]; try solve by inversion.
+      assert (res_type venv0 rx T1) as HRX. SCase "HRX". subst. eapply IHn; eauto.
+      inversion HRX as [? vx].
+
+      destruct tf as [rf|]; subst rx; try solve by inversion.
+      assert (res_type venv0 rf (TFun T1 T2)) as HRF. SCase "HRF". subst. eapply IHn; eauto.
+      inversion HRF as [? vf].
+
+      destruct (invert_abs venv0 vf T1 T2) as
+          [env1 [tenv [x0 [y0 [T3 [T4 [EF [FRX [WF [HTY [STX STY]]]]]]]]]]]. eauto.
+      (* now we know it's a closure, and we have has_type evidence *)
+
+      assert (res_type (vx::env1) res T4) as HRY.
+        SCase "HRY".
+          subst. eapply IHn. eauto. eauto.
+          (* wf_env x *) econstructor. eapply valtp_widen; eauto.
+                         eapply stpd2_extend2. eauto. eauto. eauto.
+
+      inversion HRY as [? vy].
+
+      eapply not_stuck. eapply valtp_widen; eauto. eapply stpd2_extend1. eauto.
+
+    + eapply restp_widen. eapply IHhas_type; eauto.
+      eapply stpd2_upgrade. eapply stp_to_stp2; eauto. econstructor.
+
+  - Case "TAbs".
+    remember (ttabs t e) as xe. induction H0; inversion Heqxe; subst.
+    + eapply not_stuck. eapply v_tabs; eauto.
+      eauto. eapply stpd2_upgrade. eapply stp_to_stp2. eauto. eauto. econstructor.
+    + eapply restp_widen. eapply IHhas_type; eauto.
+      eapply stpd2_upgrade. eapply stp_to_stp2; eauto. econstructor.
+
+  - Case "TApp".
+    remember (ttapp e t) as xe. induction H0; inversion Heqxe; subst.
+    +
+      remember t as T11.
+      remember (teval n venv0 e) as tf.
+
+      destruct tf as [rf|]; try solve by inversion.
+      assert (res_type venv0 rf (TAll T11 T12)) as HRF. SCase "HRF". subst. eapply IHn; eauto.
+      inversion HRF as [? vf].
+
+      subst t.
+      destruct (invert_tabs venv0 vf T11 T12) as
+          [env1 [tenv [x0 [y0 [T3 [T4 [EF [FRX [WF [HTY [STX STY]]]]]]]]]]]. eauto.
+      (* now we know it's a closure, and we have has_type evidence *)
+
+      assert (res_type ((vty venv0 T11)::env1) res (open (TVarF x0) T4)) as HRY.
+        SCase "HRY".
+          subst. eapply IHn. eauto. eauto.
+          (* wf_env x *) econstructor. eapply v_ty.
+          (* wf_env   *) eauto.
+          eapply stpd2_extend2. eapply stpd2_mem.
+          eapply stpd2_wrapf. eauto. eauto.
+      eauto.
+      inversion HRY as [? vy].
+
+      eapply not_stuck. eapply valtp_widen; eauto.
+
+    + eapply restp_widen. eapply IHhas_type; eauto.
+      eapply stpd2_upgrade. eapply stp_to_stp2; eauto. econstructor.
+
+Qed.
